\documentclass[a4paper, 10pt]{scrartcl}

\usepackage[latin1]{inputenc}

\begin{document}

\section{Exercise 903}

Given:
\[
y = \frac{\sqrt{4x + 1}}{x^{2}}
\]

Solution:
\[
u = \sqrt{4x + 1}
\]
\[
u' = \frac{4 + 0}{2\sqrt{4x + 1}} = \frac{2}{\sqrt{4x + 1}}
\]

\[
v = x^{2}
\]
\[
v' = 2x^{2-1} = 2x
\]

\[
y' = \frac{\frac{2}{\sqrt{4x + 1}}x^{2} - 2x\sqrt{4x + 1}}{(x^{2})^{2}} =
\]
\[
\frac{2}{x^{2}\sqrt{4x + 1}} - \frac{2\sqrt{4x + 1}}{x^{3}} =
\]
\[
\frac{2x - 2\sqrt{4x + 1}\sqrt{4x + 1}}{x^{3}\sqrt{4x + 1}} =
\]
\[
\frac{2x - 2(4x + 1)}{x^{3}\sqrt{4x + 1}} = \frac{2x - 8x - 2}{x^{3}\sqrt{4x + 1}} = \frac{-6x - 2}{x^{3}\sqrt{4x + 1}} =
\]
\[
-\frac{6x + 2}{x^{3}\sqrt{4x + 1}} = -\frac{2(3x + 1)}{x^{3}\sqrt{4x + 1}}
\]

Result:
\[
y' = -\frac{2(3x + 1)}{x^{3}\sqrt{4x + 1}}
\]

\end{document}
