\documentclass[a4paper, 10pt]{scrartcl}

\usepackage[latin1]{inputenc}

\begin{document}

\section{Exercise 70.1}

Given:
\[f(x) = \frac{2\cos{3x}}{x^{3}}\]

Solution:
\[u(x) = 2\cos{3x}\]
\[u'(x) = 2\cdot3(-\sin{3x}) = -6\sin{3x}\]

\[v(x) = x^{3}\]
\[v'(x) = 3x^{3 - 1} = 3x^{2}\]

\[f'(x) = \frac{x^{3}(-6\sin{3x}) - 3x^{2}2\cos{3x}}{(x^{3})^{2}} =
         \frac{-6x^{3}\sin{3x} - 6x^{2}\cos{3x}}{x^{6}}\]

\[f'(x) = \frac{-6(x\sin{3x} + \cos{3x})}{x^{4}}\]

Result:
\[f'(x) = \frac{-6(x\sin{3x} + \cos{3x})}{x^{4}}\]

\end{document}
