\documentclass[a4paper, 10pt]{scrartcl}

\usepackage[latin1]{inputenc}

\begin{document}

\section{Exercise 864}

Given:
\[
f(x) = \frac{(\sqrt{x} - 1)^{2}}{x}
\]

Solution:
\[
f'(x) = \frac{2(\sqrt{x} - 1)^{2 - 1}(\frac{1}{2\sqrt{x}} - 0)x - (\sqrt{x} - 1)^{2}\cdot1}{x^{2}} =
\]
\[
\frac{(\sqrt{x} - 1)\frac{x}{\sqrt{x}} - ((\sqrt{x})^{2} - 2\sqrt{x} + 1)}{x^{2}}
\]

Using:
\[
\frac{x}{\sqrt{x}} = \frac{x\sqrt{x}}{\sqrt{x}\sqrt{x}} = \frac{x\sqrt{x}}{x} = \sqrt{x}
\]

\[
f'(x) = \frac{(\sqrt{x} - 1)\frac{x}{\sqrt{x}} - ((\sqrt{x})^{2} - 2\sqrt{x} + 1)}{x^{2}} =
\frac{(\sqrt{x} - 1)\sqrt{x} - (x - 2\sqrt{x} + 1)}{x^{2}} =
\]
\[
\frac{\sqrt{x}\sqrt{x} - \sqrt{x} - x + 2\sqrt{x} - 1}{x^{2}} = \frac{x - \sqrt{x} - x + 2\sqrt{x} - 1}{x^{2}} = 
\frac{\sqrt{x} - 1}{x^{2}}
\]

\[
f'(x) = \frac{\sqrt{x} - 1}{x^{2}}
\]

\[
f'(0.01) = \frac{\sqrt{0.01} - 1}{0.01^{2}} = \frac{\frac{1}{10} - 1}{\frac{1}{10000}} = 10000(\frac{1}{10} - 1) =
1000 - 10000 = -9000
\]

\[
0.01\cdot f'(0.01) = 0.01\cdot(-9000) = -90
\]

Result:
\[
0.01\cdot f'(0.01) = -90
\]

\end{document}
