\documentclass[a4paper, 10pt]{scrartcl}

\usepackage[latin1]{inputenc}

\newcommand*\euler{\mathrm{e}}

\begin{document}

\section{Exercise 1029b}

Given:
\[
y = x^{2}\ln{x}
\]

Solution:
\[
(x^{2})' = 2x
\]
\[
(x^{2})'' = 2
\]
\[
(x^{2})''' = 0
\]
\[
(\ln{x})' = \frac{1}{x} = x^{-1}
\]
\[
(\ln{x})'' = -x^{-2}
\]
\[
(\ln{x})''' = -(-2)x^{-3} = 2x^{-3}
\]

\[
y''' = 0\cdot\ln{x} + 3\cdot 2\cdot x^{-1} + 3\cdot 2x\cdot (-x^{-2}) + x^{2}\cdot 2x^{-3} =
\]
\[
6x^{-1} - 6x^{-1} + 2x^{-1} = 2x^{-1} = \frac{2}{x}
\]

Result:
\[
y''' = \frac{2}{x}
\]

\section{Exercise 1029c}

Given:
\[
y = x\cos{x}
\]

Solution:
\[
(x)' = 1
\]
\[
(x)'' = 0
\]
\[
(x)''' = 0
\]
\[
(\cos{x})' = -\sin{x}
\]
\[
(\cos{x})'' = -\cos{x}
\]
\[
(\cos{x})''' = -(-\sin{x}) = \sin{x}
\]

\[
y''' = 0\cdot \cos{x} + 3\cdot 0\cdot (-\sin{x}) + 3\cdot 1\cdot (-\cos{x}) + x\sin{x} =
\]
\[
-3\cos{x} + x\sin{x} = x\sin{x} - 3\cos{x}
\]

Result:
\[
y''' = x\sin{x} - 3\cos{x}
\]

\end{document}
