\documentclass[a4paper, 10pt]{scrartcl}

\usepackage[latin1]{inputenc}

\begin{document}

\section{Exercise 36.1}

Given:
\[\lim_{x\to 1}{\frac{x^{3} - 2x + 1}{2x^{3} + 3x - 5}}\]

Solution:
\[u(x) = x^{3} - 2x + 1\]
\[u(1) = 1^{3} - 2\cdot 1 + 1 = 1 - 2 + 1 = 0\]

\[v(x) = 2x^{3} + 3x - 5\]
\[v(1) = 2\cdot 1^{3} + 3\cdot 1 - 5 = 2\cdot 1 + 3 - 5 = 2 + 3 - 5 = 0\]

\[u'(x) = 3x^{3 - 1} - 2 = 3x^{2} - 2\]
\[u'(1) = 3\cdot 1^{2} - 2 = 3 - 2 = 1\]

\[v'(x) = 2\cdot 3x^{3 - 1} + 3 = 6x^{2} + 3\]
\[v'(1) = 6\cdot 1^{2} + 3 = 6 + 3 = 9\]

\[\lim_{x\to 1}{\frac{x^{3} - 2x + 1}{2x^{3} + 3x - 5}} = \lim_{x\to 1}{\frac{u'(x)}{v'(x)}} =
        \frac{1}{9}\]

Result:
\[\lim_{x\to 1}{\frac{x^{3} - 2x + 1}{2x^{3} + 3x - 5}} = \frac{1}{9}\]

\end{document}
