\documentclass[a4paper, 10pt]{scrartcl}

\usepackage[latin1]{inputenc}

\begin{document}

\section{Exercise 68.9a}

Given:
\[y(\theta) = \frac{2}{\theta^{2}} + 2\ln{2\theta} -
              2(\cos{5\theta} + 3\sin{2\theta}) - \frac{2}{e^{3\theta}}\]

Solution:
\[y(\theta) = 2\theta^{-2} + 2\ln{2\theta} -
              2\cos{5\theta} - 6\sin{2\theta} - 2e^{-3\theta}\]

\[y'(\theta) = 2(-2)\theta^{-2 - 1} + 2\frac{1}{\theta} -
              2\cdot5\cdot(-\sin{5\theta}) - 6\cdot2\cdot \cos{2\theta} - 2(-3)e^{-3\theta}\]

\[y'(\theta) = -4\theta^{-3} + \frac{2}{\theta} +
              10\sin{5\theta} - 12\cos{2\theta} + 6e^{-3\theta}\]

\[y'(\theta) = -\frac{4}{\theta^{3}} + \frac{2}{\theta} +
              10\sin{5\theta} - 12\cos{2\theta} + \frac{6}{e^{3\theta}}\]

Result:
\[y'(\theta) = -\frac{4}{\theta^{3}} + \frac{2}{\theta} +
              10\sin{5\theta} - 12\cos{2\theta} + \frac{6}{e^{3\theta}}\]

\section{Exercise 68.9b}

Given:
\[\theta = \frac{\pi}{2}\]
\[y'(\theta) = -\frac{4}{\theta^{3}} + \frac{2}{\theta} +
              10\sin{5\theta} - 12\cos{2\theta} + \frac{6}{e^{3\theta}}\]

Solution:
\[y'(\frac{\pi}{2}) = -\frac{4}{(\frac{\pi}{2})^{3}} + \frac{2}{\frac{\pi}{2}} +
              10\sin{5\frac{\pi}{2}} - 12\cos{2\frac{\pi}{2}} + \frac{6}{e^{3\frac{\pi}{2}}}\]

\[y'(\frac{\pi}{2}) = -\frac{4}{(\frac{\pi^{3}}{8})} + \frac{4}{\pi} +
              10\sin{\frac{\pi}{2}} - 12\cos{\pi} + \frac{6}{e^{3\frac{\pi}{2}}}\]

\[y'(\frac{\pi}{2}) = -\frac{32}{\pi^{3}} + \frac{4}{\pi} +
              10 + 12 + \frac{6}{e^{3\frac{\pi}{2}}}\]

\[y'(\frac{\pi}{2}) = -\frac{32}{\pi^{3}} + \frac{4}{\pi} +
              22 + \frac{6}{e^{3\frac{\pi}{2}}} = 22,29509019 \approx 22,3 \]

Result:
\[y'(\frac{\pi}{2}) \approx 22,3\]

\end{document}
