\documentclass[a4paper, 10pt]{scrartcl}

\usepackage[latin1]{inputenc}

\newcommand*\euler{\mathrm{e}}

\begin{document}

\section{Exercise 956a}

Given:
\[
y = \euler^{-x}(\sin{x} + \cos{x})
\]

Solution:
\[
y' = -\euler^{-x}(\sin{x} + \cos{x}) + \euler^{-x}(\cos{x} - \sin{x}) =
\]
\[
\euler^{-x}(-\sin{x} - \cos{x} + \cos{x} - \sin{x}) = \euler^{-x}\cdot(-2\cdot\sin{x}) = -2\euler^{-x}\sin{x}
\]

Result:
\[
y' = -2\euler^{-x}\sin{x}
\]

\section{Exercise 956b}

Given:
\[
y = \ln{(\euler^{-x} + x\euler^{-x})}
\]

Solution:
\[
y' = \frac{1}{\euler^{-x} + x\euler^{-x}}\cdot\left(-\euler^{-x} + 1\euler^{-x} + x(-\euler^{-x})\right) =
\]
\[
\frac{1}{\euler^{-x} + x\euler^{-x}}\cdot(-x\euler^{-x}) = -\frac{x}{\euler^{-x} + x\euler^{-x}}\cdot\euler^{-x} =
\]
\[
-\frac{x}{\euler^{-x}(1 + x)}\cdot\euler^{-x} = -\frac{x}{1 + x}
\]

Result:
\[
y' = -\frac{x}{1 + x}
\]

\end{document}
