\documentclass[a4paper, 10pt]{scrartcl}

\usepackage[latin1]{inputenc}

\begin{document}

\section{Exercise 66.2}

\[f(x) = \cos{8x}\sin{2x}\]

Using:
\[\cos{\alpha}\sin{\beta} = \frac{1}{2}(\sin{(\alpha + \beta)} - \sin{(\alpha - \beta)})\]

\[f(x) = \frac{1}{2}(\sin{(8x + 2x)} - \sin{(8x - 2x)})\]
\[f(x) = \frac{1}{2}(\sin{10x} - \sin{6x})\]

Result:
\[f(x) = \cos{8x}\sin{2x} = \frac{1}{2}(\sin{10x} - \sin{6x})\]

\section{Exercise 66.3}

\[f(t) = 2\sin{7t}\sin{3t}\]

Using:
\[\sin{\alpha}\sin{\beta} = -\frac{1}{2}(\cos{(\alpha + \beta)} - \cos{(\alpha - \beta)})\]

\[f(t) = 2\left(-\frac{1}{2}(\cos{(7t + 3t)} - \cos{(7t - 3t)})\right)\]
\[f(t) = 2\left(-\frac{1}{2}(\cos{10t} - \cos{4t})\right)\]
\[f(t) = -(\cos{10t} - \cos{4t})\]
\[f(t) = -\cos{10t} + \cos{4t} = \cos{4t} - \cos{10t}\]

Result:
\[f(t) = 2\sin{7t}\sin{3t} = \cos{4t} - \cos{10t}\]

\section{Exercise 66.4}

\[f(\theta) = 4\cos{3\theta}\cos{\theta}\]

Using:
\[\cos{\alpha}\cos{\beta} = \frac{1}{2}(\cos{(\alpha + \beta)} + \cos{(\alpha - \beta)})\]

\[f(\theta) = 4\left(\frac{1}{2}(\cos{(3\theta + \theta)} + \cos{(3\theta - \theta)})\right)\]
\[f(\theta) = 4\left(\frac{1}{2}(\cos{4\theta} + \cos{2\theta})\right)\]
\[f(\theta) = 2(\cos{4\theta} + \cos{2\theta})\]

Result:
\[f(\theta) = 4\cos{3\theta}\cos{\theta} = 2(\cos{4\theta} + \cos{2\theta})\]

\end{document}
