\documentclass[a4paper, 10pt]{scrartcl}

\usepackage[latin1]{inputenc}

\begin{document}

\section{Exercise 851a}

Given:
\[
y = x + 2\sqrt{x}
\]

Solution:
\[
y' = 1 + 2\frac{1}{2\sqrt{x}} = 1 + \frac{1}{\sqrt{x}}
\]

Result:
\[
y' = 1 + \frac{1}{\sqrt{x}}
\]

\section{Exercise 851b}

Given:
\[
y = (\sqrt{a} - \sqrt{x})^{2}
\]

Solution:
\[
y' = 2(\sqrt{a} - \sqrt{x})^{2 - 1}\cdot(0 - \frac{1}{2\sqrt{x}}) = -\frac{1}{\sqrt{x}}(\sqrt{a} - \sqrt{x}) =
\]
\[
-\frac{\sqrt{a}}{\sqrt{x}} + \frac{\sqrt{x}}{\sqrt{x}} = -\sqrt{\frac{a}{x}} + 1 = 1 - \sqrt{\frac{a}{x}}
\]

Result:
\[
y' = 1 - \sqrt{\frac{a}{x}}
\]

\end{document}
