\documentclass[a4paper, 10pt]{scrartcl}

\usepackage[latin1]{inputenc}

\begin{document}

\section{Exercise 68.3a}

Given:
\[f(x) = 2\sqrt{x}\]

Solution:
\[f(x) = 2\sqrt{x} = 2x^{\frac{1}{2}}\]

\[f'(x) = 2\cdot\frac{1}{2}\cdot x^{\frac{1}{2} - 1}\]
\[f'(x) = x^{-\frac{1}{2}} = \frac{1}{x^\frac{1}{2}} = \frac{1}{\sqrt{x}}\]

Result:
\[f'(x) = \frac{1}{\sqrt{x}}\]

\section{Exercise 68.3b}

Given:
\[f(x) = 3\sqrt[3]{x^5}\]

Solution:
\[f(x) = 3\sqrt[3]{x^5} = 3x^{\frac{5}{3}}\]
\[f'(x) = 3\cdot\frac{5}{3}\cdot x^{\frac{5}{3} - 1} = 5x^{\frac{2}{3}}\]
\[f'(x) = 5\sqrt[3]{x^2}\]

Result:
\[f'(x) = 5\sqrt[3]{x^2}\]

\section{Exercise 68.3c}

Given:
\[f(x) = \frac{4}{\sqrt{x}}\]

Solution:
\[f(x) = \frac{4}{\sqrt{x}} = 4x^{-\frac{1}{2}}\]
\[f'(x) = 4\cdot(-\frac{1}{2})\cdot x^{-\frac{1}{2} - 1} = -2x^{-\frac{3}{2}}\]
\[f'(x) = \frac{-2}{x^{\frac{3}{2}}} = \frac{-2}{\sqrt{x^{3}}} = -\frac{2}{\sqrt{x^{3}}}\]

Result:
\[f'(x) = -\frac{2}{\sqrt{x^{3}}}\]

\end{document}
