\documentclass[a4paper, 10pt]{scrartcl}

\usepackage[latin1]{inputenc}

\newcommand*\euler{\mathrm{e}}

\begin{document}

\section{Exercise 1028a}

Given:
\[
y = \euler^{x}\cos{x}
\]

Solution:
\[
(\euler^{x})' = \euler^{x}
\]
\[
(\euler^{x})'' = \euler^{x}
\]
\[
(\cos{x})' = -\sin{x}
\]
\[
(\cos{x})'' = -\cos{x}
\]

\[
y'' = \euler^{x}\cos{x} + 2\euler^{x}(-\sin{x}) + \euler^{x}(-\cos{x}) =
\]
\[
\euler^{x}(\cos{x} - 2\sin{x} - \cos{x}) = -2\euler^{x}\sin{x}
\]

Result:
\[
y'' = -2\euler^{x}\sin{x}
\]

\section{Exercise 1028b}

Given:
\[
y = a^{x}x^{3}
\]

Solution:
\[
(a^{x})' = a^{x}\ln{a}
\]
\[
(a^{x})'' = a^{x}\ln{a}\ln{a} = a^{x}\ln^{2}{x}
\]
\[
(x^{3})' = 3x^{2}
\]
\[
(x^{3})'' = 6x
\]

\[
y'' = a^{x}\ln^{2}{x}(x^{3}) + 2a^{x}\ln{a}(3x^{2}) + a^{x}6x =
\]
\[
a^{x}(x^{3}\ln^{2}{x} + 6x^{2}\ln{a} + 6x) = a^{x}x(x^{2}\ln^{2}{x} + 6x\ln{a} + 6)
\]

Result:
\[
y'' = a^{x}x(x^{2}\ln^{2}{x} + 6x\ln{a} + 6)
\]

\section{Exercise 1028c}

Given:
\[
y = x^{2}\sin{x}
\]

Solution:
\[
(x^{2})' = 2x
\]
\[
(x^{2})'' = 2
\]
\[
(\sin{x})' = \cos{x}
\]
\[
(\sin{x})'' = -\sin{x}
\]

\[
y'' = 2\sin{x} + 2\cdot 2x\cdot\cos{x} + x^{2}(-\sin{x}) =
\]
\[
2\sin{x} + 4x\cos{x} - x^{2}\sin{x} = \sin{x}(2 - x^{2}) + 4x\cos{x}
\]

Result:
\[
y'' = \sin{x}(2 - x^{2}) + 4x\cos{x}
\]

\end{document}
