\documentclass[a4paper, 10pt]{scrartcl}

\usepackage[latin1]{inputenc}

\begin{document}

\section{Exercise 938a}

Given:
\[
y = \ln{x} - \frac{2}{x} - \frac{1}{2x^{2}}
\]

Solution:
\[
y = \ln{x} - \frac{2}{x} - \frac{1}{2x^{2}} = \ln{x} - 2x^{-1} - \frac{1}{2}x^{-2}
\]

\[
y' = \frac{1}{x} - 2(-1)x^{-1 - 1} - \frac{1}{2}(-2)x^{-2 - 1} = \frac{1}{x} + 2x^{-2} + x^{-3} =
\]
\[
\frac{1}{x} + \frac{2}{x^{2}} + \frac{1}{x^{3}} = \frac{x^{2} + 2x + 1}{x^{3}} = \frac{(x + 1)^{2}}{x^{3}}
\]

Result:
\[
y' = \frac{(x + 1)^{2}}{x^{3}}
\]

\section{Exercise 938b}

Given:
\[
y = \ln{x^{2} + 2x}
\]

Solution:

Result:

\end{document}
