\documentclass[a4paper, 10pt]{scrartcl}

\usepackage[latin1]{inputenc}

\begin{document}

\section{Exercise 1022a}

Given:
\[
y = \cos^{2}{x}
\]

Solution:
\[
y' = 2\cos{x}(-\sin{x}) = -2\cos{x}\sin{x}
\]
\[
y'' = -2(-\sin{x}\sin{x} + \cos{x}\cos{x}) = -2\cos{(x + x)} = -2\cos{2x}
\]
\[
y''' = -2(-\sin{2x})2 = -4\sin{2x}
\]

Result:
\[
y''' = -4\sin{2x}
\]

\section{Exercise 1022b}

Given:
\[
y = \frac{1}{x^{2}}
\]

Solution:
\[
y = \frac{1}{x^{2}} = x^{-2}
\]
\[
y' = -2x^{-3}
\]
\[
y'' = -2\cdot (-3)x^{-4} = 6x^{-4}
\]
\[
y''' = 6\cdot (-4)x^{-5} = -24x^{-5} = -\frac{24}{x^{5}}
\]

Result:
\[
y''' = -\frac{24}{x^{5}}
\]

\section{Exercise 1022c}

Given:
\[
y = x\sin{x}
\]

Solution:
\[
y' = \sin{x} + x\cos{x}
\]
\[
y'' = \cos{x} + (\cos{x} + x(-\sin{x})) = 2\cos{x} - x\sin{x}
\]
\[
y''' = 2(-\sin{x}) - (\sin{x} + x\cos{x}) = -2\sin{x} - \sin{x} - x\cos{x} = -3\sin{x} - x\cos{x}
\]

Result:
\[
y''' = -3\sin{x} - x\cos{x}
\]

\end{document}
