\documentclass[a4paper, 10pt]{scrartcl}

\usepackage[latin1]{inputenc}

\begin{document}

\section{Exercise 1011}

Given:
\[
y = 4\ln{(\sqrt{x - 4} + \sqrt{x})} + \sqrt{x^{2} - 4x}
\]

Solution:
\[
(\sqrt{x^{2} - 4x})' = \frac{1}{2\sqrt{x^{2} - 4x}}(2x - 4) = \frac{x - 2}{\sqrt{x^{2} - 4x}}
\]
\[
(4\ln{(\sqrt{x - 4} + \sqrt{x})})' = 4\frac{1}{\sqrt{x - 4} + \sqrt{x}}\left(\frac{1}{2\sqrt{x - 4}} + \frac{1}{2\sqrt{x}}\right) =
\]
\[
\frac{2}{\sqrt{x - 4} + \sqrt{x}}\left(\frac{1}{\sqrt{x - 4}} + \frac{1}{\sqrt{x}}\right) =
\]
\[
\frac{2}{\sqrt{x - 4} + \sqrt{x}}\frac{\sqrt{x} + \sqrt{x - 4}}{\sqrt{x}\sqrt{x - 4}} = \frac{2}{\sqrt{x}\sqrt{x - 4}}
\]

\[
y' = (4\ln{(\sqrt{x - 4} + \sqrt{x})})' + (\sqrt{x^{2} - 4x})' =
\]
\[
\frac{2}{\sqrt{x}\sqrt{x - 4}} + \frac{x - 2}{\sqrt{x^{2} - 4x}} = \frac{2}{\sqrt{x^{2} - 4x}} + \frac{x - 2}{\sqrt{x^{2} - 4x}} =
\]
\[
\frac{2 + x - 2}{\sqrt{x^{2} - 4x}} = \frac{x}{\sqrt{x^{2} - 4x}}
\]

Result:
\[
y' = \frac{x}{\sqrt{x^{2} - 4x}}
\]

\end{document}
