\documentclass[a4paper, 10pt]{scrartcl}

\usepackage[latin1]{inputenc}

\begin{document}

\section{Exercise 67.6a}

\[f(x) = \frac{\sin{4x} - \sin{2x}}{\cos{4x} + \cos{2x}}\]

Using:
\[\sin{\alpha} - \sin{\beta} = 2\cos{\frac{\alpha + \beta}{2}}\sin{\frac{\alpha - \beta}{2}}\]
\[\cos{\alpha} + \cos{\beta} = 2\cos{\frac{\alpha + \beta}{2}}\cos{\frac{\alpha - \beta}{2}}\]

\[f(x) = \frac{2\cos{\frac{4x + 2x}{2}}\sin{\frac{4x - 2x}{2}}}
              {2\cos{\frac{4x + 2x}{2}}\cos{\frac{4x - 2x}{2}}}\]

\[f(x) = \frac{2\cos{\frac{6x}{2}}\sin{\frac{2x}{2}}}
              {2\cos{\frac{6x}{2}}\cos{\frac{2x}{2}}}\]

\[f(x) = \frac{2\cos{3x}\sin{x}}
              {2\cos{3x}\cos{x}}\]

\[f(x) = \frac{\cos{3x}\sin{x}}
              {\cos{3x}\cos{x}}\]

\[f(x) = \frac{\sin{x}}{\cos{x}} = \tan{x}\]

Solution:
\[f(x) = \frac{\sin{4x} - \sin{2x}}{\cos{4x} + \cos{2x}} = \tan{x}\]

\section{Exercise 67.6b}

\[f(x) = \frac{1}{2}(\sin{(5x - \alpha)} - \sin{(x + \alpha)})\]

Using:
\[\sin{\alpha} - \sin{\beta} = 2\cos{\frac{\alpha + \beta}{2}}\sin{\frac{\alpha - \beta}{2}}\]

\[f(x) = \frac{1}{2}\left(2\cos{\frac{(5x - \alpha) + (x + \alpha)}{2}}
                      \sin{\frac{(5x - \alpha) - (x + \alpha)}{2}}\right)\]

\[f(x) = \cos{\frac{(5x - \alpha) + (x + \alpha)}{2}}
         \sin{\frac{(5x - \alpha) - (x + \alpha)}{2}}\]

\[f(x) = \cos{\frac{5x - \alpha + x + \alpha}{2}}
         \sin{\frac{5x - \alpha - x - \alpha}{2}}\]

\[f(x) = \cos{\frac{6x}{2}}\sin{\frac{4x - 2\alpha}{2}}\]

\[f(x) = \cos{3x}\sin{(2x - \alpha)}\]

Solution:
\[f(x) = \frac{1}{2}(\sin{(5x - \alpha)} - \sin{(x + \alpha)}) = \cos{3x}\sin{(2x - \alpha)}\]

\end{document}
