\documentclass[a4paper, 10pt]{scrartcl}

\usepackage[latin1]{inputenc}

\begin{document}

\section{Exercise 68.4a}

Given:
\[f(x) = \frac{-3}{\sqrt[3]{x}}\]

Solution:
\[f(x) = \frac{-3}{\sqrt[3]{x}} = \frac{-3}{x^{\frac{1}{3}}} = -3x^{-\frac{1}{3}}\]

\[f'(x) = -3\cdot(-\frac{1}{3})\cdot x^{-\frac{1}{3} - 1} = x^{-\frac{4}{3}}\]
\[f'(x) = x^{-\frac{4}{3}} = \frac{1}{x^{\frac{4}{3}}} = \frac{1}{\sqrt[3]{x^{4}}}\]

Result:
\[f'(x) = \frac{1}{\sqrt[3]{x^{4}}}\]

\section{Exercise 68.4b}

Given:
\[f(x) = (x - 1)^{2}\]

Solution:
\[f'(x) = 2(x - 1)^{2 - 1} = 2(x - 1)^{1} = 2(x - 1)\]

Result:
\[f'(x) = 2(x - 1)\]

\section{Exercise 68.4c}

Given:
\[f(x) = 2\sin{3x}\]

Solution:
\[f'(x) = 2\cdot3\cdot \cos{3x} = 6\cos{3x}\]

Result:
\[f'(x) = 6\cos{3x}\]

\end{document}
