\documentclass[a4paper, 10pt]{scrartcl}

\usepackage[latin1]{inputenc}

\newcommand*\euler{\mathrm{e}}

\begin{document}

\section{Exercise 1025a}

Given:
\[
y = \euler^{-\frac{x}{a}}
\]

Solution:
\[
y' = -\frac{1}{a}\euler^{-\frac{x}{a}}
\]
\[
y'' = -\frac{1}{a}(-\frac{1}{a})\euler^{-\frac{x}{a}} = \frac{1}{a^{2}}\euler^{-\frac{x}{a}}
\]
\[
y''' = \frac{1}{a^{2}}(-\frac{1}{a})\euler^{-\frac{x}{a}} = -\frac{1}{a^{3}}\euler^{-\frac{x}{a}}
\]
\[
y^{(4)} = -\frac{1}{a^{3}}(-\frac{1}{a})\euler^{-\frac{x}{a}} = \frac{1}{a^{4}}\euler^{-\frac{x}{a}}
\]
\[
y^{(5)} = \frac{1}{a^{4}}(-\frac{1}{a})\euler^{-\frac{x}{a}} = -\frac{1}{a^{5}}\euler^{-\frac{x}{a}}
\]
\[
y^{(n)} = (-1)^{n}\frac{1}{a^{n}}\euler^{-\frac{x}{a}}
\]

Result:
\[
y^{(n)} = (-1)^{n}\frac{1}{a^{n}}\euler^{-\frac{x}{a}}
\]

\end{document}
