\documentclass[a4paper, 10pt]{scrartcl}

\usepackage[latin1]{inputenc}

\begin{document}

\section{Exercise 1012}

Given:
\[
s = \frac{1}{4}\tan^{4}{t} - \frac{1}{2}\tan^{2}{t} - \ln{(\cos{t})}
\]

Solution:
\[
(\frac{1}{4}\tan^{4}{t})' = \frac{1}{4}\cdot 4\tan^{3}{t}\frac{1}{\cos^{2}{t}} = \frac{\tan^{3}{t}}{\cos^{2}{t}} = \frac{\sin^{3}{t}}{\cos^{5}{t}}
\]

\[
(\frac{1}{2}\tan^{2}{t})' = \frac{1}{2}\cdot 2\tan{t}\frac{1}{\cos^{2}{t}} = \frac{\tan{t}}{\cos^{2}{t}} = \frac{\sin{t}}{\cos^{3}{t}}
\]

\[
(\ln{(\cos{t})})' = \frac{1}{\cos{t}}\cdot(-\sin{t}) = \frac{-\sin{t}}{\cos{t}}
\]

\[
s' = \frac{\sin^{3}{t}}{\cos^{5}{t}} - \frac{\sin{t}}{\cos^{3}{t}} - (\frac{-\sin{t}}{\cos{t}}) =
\]
\[
\frac{\sin^{3}{t}}{\cos^{5}{t}} - \frac{\sin{t}}{\cos^{3}{t}} + \frac{\sin{t}}{\cos{t}} =
\]
\[
\frac{\sin^{3}{t} - \sin{t}\cos^{2}{t} + \sin{t}\cos^{4}{t}}{\cos^{5}{t}} = \frac{\sin^{3}{t} + \sin{t}\cos^{2}{t}(-1 + \cos^{2}{t})}{\cos^{5}{t}} =
\]
\[
\frac{\sin^{3}{t} + \sin{t}\cos^{2}{t}(-\sin^{2}{t})}{\cos^{5}{t}} =
\]
\[
\frac{\sin^{3}{t} - \sin^{3}{t}\cos^{2}{t}}{\cos^{5}{t}} = \frac{\sin^{3}{t}(1 - \cos^{2}{t})}{\cos^{5}{t}} =
\]
\[
\frac{\sin^{3}{t}\sin^{2}{t}}{\cos^{5}{t}} = \frac{\sin^{5}{t}}{\cos^{5}{t}} = \tan^{5}{t}
\]

Result:
\[
s' = \tan^{5}{t}
\]

\end{document}
