\documentclass[a4paper, 10pt]{scrartcl}

\usepackage[latin1]{inputenc}

\begin{document}

\section{Exercise 889}

Given:
\[
y = x\sqrt{x^{2} - 1}
\]

Solution:
\[
y' = 1\sqrt{x^{2} - 1} + x\frac{2x - 0}{2\sqrt{x^{2} - 1}} = \sqrt{x^{2} - 1} + \frac{x^{2}}{\sqrt{x^{2} - 1}} =
\]
\[
\frac{\sqrt{x^{2} - 1}\sqrt{x^{2} - 1} + x^{2}}{\sqrt{x^{2} - 1}} =
\]
\[
\frac{x^{2} - 1 + x^{2}}{\sqrt{x^{2} - 1}} = \frac{2x^{2} - 1}{\sqrt{x^{2} - 1}}
\]

Result:
\[
y' = \frac{2x^{2} - 1}{\sqrt{x^{2} - 1}}
\]

\section{Exercise 890}

Given:
\[
y = \frac{\sqrt{2x - 1}}{x}
\]

Solution:
\[
y = \frac{\sqrt{2x - 1}}{x} = \sqrt{2x - 1}x^{-1}
\]
\[
y' = \frac{2 - 0}{2\sqrt{2x - 1}}x^{-1} + \sqrt{2x - 1}(-1)x^{-1 - 1} = \frac{1}{x\sqrt{2x - 1}} - \frac{\sqrt{2x - 1}}{x^{2}} =
\]
\[
\frac{x - \sqrt{2x - 1}\sqrt{2x - 1}}{x^{2}\sqrt{2x - 1}} =
\]
\[
\frac{x - (2x - 1)}{x^{2}\sqrt{2x - 1}} = \frac{x - 2x + 1}{x^{2}\sqrt{2x - 1}} =
\]
\[
\frac{-x + 1}{x^{2}\sqrt{2x - 1}} = \frac{1 - x}{x^{2}\sqrt{2x - 1}}
\]

Result:
\[
y' = \frac{1 - x}{x^{2}\sqrt{2x - 1}}
\]

\section{Exercise 891}

Given:
\[
s = a\cos^{2}{\frac{t}{a}}
\]

Solution:
\[
s' = a2\cos^{2 - 1}{\frac{t}{a}}(-\sin{\frac{t}{a}})\frac{1}{a} = -2\cos{\frac{t}{a}}\sin{\frac{t}{a}} = -\sin{\frac{2t}{a}}
\]

Result:
\[
s' = -\sin{\frac{2t}{a}}
\]

\end{document}
