\documentclass[a4paper, 10pt]{scrartcl}

\usepackage[latin1]{inputenc}

\begin{document}

\section{Exercise 863}

Given:
\[
f(x) = x^{2} - \frac{1}{2x^{2}}
\]

Solution:
\[
f(x) = x^{2} - \frac{1}{2x^{2}} = x^{2} - \frac{1}{2}x^{-2}
\]

\[
f'(x) = 2x^{2 - 1} - \frac{1}{2}(-2)x^{-2 - 1} = 2x + x^{-3} = 2x + \frac{1}{x^{3}}
\]

\[
f'(x) = 2x + \frac{1}{x^{3}}
\]

\[
f'(2) = 2\cdot2 + \frac{1}{2^{3}} = 4 + \frac{1}{8} = 4\frac{1}{8} = \frac{33}{8}
\]
\[
f'(-2) = 2(-2) + \frac{1}{(-2)^{3}} = -4 + \frac{1}{-8} = -4 - \frac{1}{8} = -4\frac{1}{8} = -\frac{33}{8}
\]

\[
f'(2) - f'(-2) = \frac{33}{8} - (-\frac{33}{8}) = \frac{33}{8} + \frac{33}{8} = \frac{33}{4} = 8\frac{1}{4}
\]

Result:
\[
f'(2) - f'(-2) = 8\frac{1}{4}
\]

\end{document}
