\documentclass[a4paper, 10pt]{scrartcl}

\usepackage[latin1]{inputenc}

\begin{document}

\section{Exercise 1021a}

Given:
\[
y = \sin^{2}{x}
\]

Solution:
\[
y' = 2\sin{x}\cos{x}
\]
\[
y'' = 2(\cos{x}\cos{x} + \sin{x}(-\sin{x})) = 2(\cos{x}\cos{x} - \sin{x}\sin{x}) = 2\cos{(x + x)} = 2\cos{2x}
\]

Result:
\[
y'' = 2\cos{2x}
\]

\section{Exercise 1021b}

Given:
\[
y = \tan{x}
\]

Solution:
\[
y' = \frac{1}{\cos^{2}{x}} = \cos^{-2}{x}
\]
\[
y'' = -2\cos^{-2 - 1}{x}(-\sin{x}) = 2\cos^{-3}{x}\sin{x} = \frac{2\sin{x}}{\cos^{3}{x}} = \frac{2\tan{x}}{\cos^{2}{x}}
\]

Result:
\[
y'' = \frac{2\tan{x}}{\cos^{2}{x}}
\]

\section{Exercise 1021c}

Given:
\[
y = \sqrt{1 + x^{2}}
\]

Solution:
\[
y' = \frac{1}{2\sqrt{1 + x^{2}}}2x = \frac{x}{\sqrt{1 + x^{2}}}
\]
\[
y'' = \frac{1\sqrt{1 + x^{2}} - x\frac{2x}{2\sqrt{1 + x^{2}}}}{(\sqrt{1 + x^{2}})^{2}} =
\]
\[
\frac{\sqrt{1 + x^{2}} - \frac{x^{2}}{\sqrt{1 + x^{2}}}}{1 + x^{2}} =
\]
\[
\frac{\sqrt{1 + x^{2}}\sqrt{1 + x^{2}} - x^{2}}{(1 + x^{2})\sqrt{1 + x^{2}}} =
\]
\[
\frac{1 + x^{2} - x^{2}}{(1 + x^{2})(1 + x^{2})^{\frac{1}{2}}} = \frac{1}{(1 + x^{2})^{\frac{3}{2}}}
\]

Result:
\[
y'' = \frac{1}{(1 + x^{2})^{\frac{3}{2}}}
\]

\end{document}
