\documentclass[a4paper, 10pt]{scrartcl}

\usepackage[latin1]{inputenc}

\begin{document}

\section{Exercise 67.4}

\[f(t) = \frac{1}{8}(\cos{5t} - \cos{t})\]

Using:
\[\cos{\alpha} - \cos{\beta} = -2\sin{\frac{\alpha + \beta}{2}}\sin{\frac{\alpha - \beta}{2}}\]

\[f(t) = \frac{1}{8}(-2\sin{\frac{5t + t}{2}}\sin{\frac{5t - t}{2}})\]
\[f(t) = -\frac{1}{4}\sin{\frac{5t + t}{2}}\sin{\frac{5t - t}{2}}\]
\[f(t) = -\frac{1}{4}\sin{\frac{6t}{2}}\sin{\frac{4t}{2}}\]
\[f(t) = -\frac{1}{4}\sin{3t}\sin{2t}\]

Solution:
\[f(t) = \frac{1}{8}(\cos{5t} - \cos{t}) = -\frac{1}{4}\sin{3t}\sin{2t}\]

\section{Exercise 67.5}

\[f(x) = \frac{1}{2}(\cos{\frac{\pi}{3}} + \cos{\frac{\pi}{4}})\]

Using:
\[\cos{\alpha} + \cos{\beta} = 2\cos{\frac{\alpha + \beta}{2}}\cos{\frac{\alpha - \beta}{2}}\]

\[f(x) = \frac{1}{2}(2\cos{\frac{\frac{\pi}{3} + \frac{\pi}{4}}{2}}\cos{\frac{\frac{\pi}{3} - \frac{\pi}{4}}{2}})\]
\[f(x) = \cos{\frac{\frac{\pi}{3} + \frac{\pi}{4}}{2}}\cos{\frac{\frac{\pi}{3} - \frac{\pi}{4}}{2}}\]

Note:
\[\frac{\pi}{3} + \frac{\pi}{4} = \frac{4\pi + 3\pi}{12} = \frac{7\pi}{12}\]
\[\frac{\pi}{3} - \frac{\pi}{4} = \frac{4\pi - 3\pi}{12} = \frac{\pi}{12}\]

\[f(x) = \cos{\frac{\frac{7\pi}{12}}{2}}\cos{\frac{\frac{\pi}{12}}{2}}\]
\[f(x) = \cos{\frac{7\pi}{24}}\cos{\frac{\pi}{24}}\]

Solution:
\[f(x) = \frac{1}{2}(\cos{\frac{\pi}{3}} + \cos{\frac{\pi}{4}}) = \cos{\frac{7\pi}{24}}\cos{\frac{\pi}{24}}\]

\end{document}
