\documentclass[a4paper, 10pt]{scrartcl}

\usepackage[latin1]{inputenc}

\begin{document}

\section{Exercise 858a}

Given:
\[
y = \frac{\cos{x}}{x^{2}}
\]

Solution:
\[
y' = \frac{(-\sin{x})x^{2} - 2x\cos{x}}{(x^{2})^{2}} = \frac{-x^{2}\sin{x} - 2x\cos{x}}{x^{4}} =
\]
\[
\frac{-x(x\sin{x} + 2\cos{x})}{x^{4}} = \frac{-(x\sin{x} + 2\cos{x})}{x^{3}}
\]

Result:
\[
y' = \frac{-(x\sin{x} + 2\cos{x})}{x^{3}}
\]

\section{Exercise 858b}

Given:
\[
y = \frac{x^{2}}{x^{2} + 1}
\]

Solution:
\[
y' = \frac{2x(x^{2} + 1) - (2x + 0)x^{2}}{(x^{2} + 1)^{2}} = \frac{2x^{3} + 2x - 2x^{3}}{(x^{2} + 1)^{2}} = \frac{2x}{(x^{2} + 1)^{2}}
\]

Result:
\[
y' = \frac{2x}{(x^{2} + 1)^{2}}
\]

\end{document}
