\documentclass[a4paper, 10pt]{scrartcl}

\usepackage[latin1]{inputenc}

\begin{document}

\section{Exercise 65.3}

Given:
\[f(\theta) = V_{3}\cos{3\theta}\]
\[V_{3} = 1\]

Using:
\[\cos{(\alpha + \beta)} = \cos{\alpha}\cos{\beta} - \sin{\alpha}\sin{\beta}\]

Solution:
\[f(\theta) = V_{3}\cos{3\theta} = 1\cos{3\theta} = \cos{(\theta + 2\theta)}\]
\[\cos{(\theta + 2\theta)} = \cos{\theta}\cos{2\theta} - \sin{\theta}\sin{2\theta}\]

Using:
\[\cos{2\alpha} = 2\cos^{2}{\alpha} - 1\]
\[\sin{2\alpha} = 2\sin{\alpha}\cos{\alpha}\]

\[\cos{\theta}\cos{2\theta} - \sin{\theta}\sin{2\theta} =
\cos{\theta}(2\cos^{2}{\theta} - 1) - \sin{\theta}(2\sin{\theta}\cos{\theta})\]
\[2\cos^{3}{\theta} - \cos{\theta} - 2\sin^{2}{\theta}\cos{\theta}\]

Using:
\[\sin^{2}{\alpha} + \cos^{2}{\alpha} = 1\]
\[\sin^{2}{\alpha} = 1 - \cos^{2}{\alpha}\]

\[2\cos^{3}{\theta} - \cos{\theta} - 2(1 - \cos^{2}{\theta})\cos{\theta}\]
\[2\cos^{3}{\theta} - \cos{\theta} - 2(\cos{\theta} - \cos^{3}{\theta})\]
\[2\cos^{3}{\theta} - \cos{\theta} - 2\cos{\theta} + 2\cos^{3}{\theta}\]
\[4\cos^{3}{\theta} - 3\cos{\theta}\]

Result:
\[f(\theta) = V_{3}\cos{3\theta} = 4\cos^{3}{\theta} - 3\cos{\theta}\]

\end{document}
