\documentclass[a4paper, 10pt]{scrartcl}

\usepackage[latin1]{inputenc}

\begin{document}

\section{Exercise 893}

Given:
\[
f(t) = \sqrt{a^{2} + b^{2} - 2ab\cos{t}}
\]

Solution:
\[
f'(t) = \frac{0 + 0 - 2ab(-\sin{t})}{2\sqrt{a^{2} + b^{2} - 2ab\cos{t}}} = \frac{ab\sin{t}}{\sqrt{a^{2} + b^{2} - 2ab\cos{t}}}
\]

\[
f'(t) = \frac{ab\sin{t}}{\sqrt{a^{2} + b^{2} - 2ab\cos{t}}}
\]

\[
f'(\frac{\pi}{2}) = \frac{ab\sin{\frac{\pi}{2}}}{\sqrt{a^{2} + b^{2} - 2ab\cos{\frac{\pi}{2}}}} =
\frac{ab\cdot1}{\sqrt{a^{2} + b^{2} - 2ab\cdot0}} = \frac{ab}{\sqrt{a^{2} + b^{2}}}
\]

\[
f'(\pi) = \frac{ab\sin{\pi}}{\sqrt{a^{2} + b^{2} - 2ab\cos{\pi}}} =
\frac{ab\cdot0}{\sqrt{a^{2} + b^{2} - 2ab\cos{\pi}}} = \frac{ab\cdot0}{\sqrt{a^{2} + b^{2} - 2ab(-1)}} = 0
\]

\[
f'(\frac{3\pi}{2}) = \frac{ab\sin{\frac{3\pi}{2}}}{\sqrt{a^{2} + b^{2} - 2ab\cos{\frac{3\pi}{2}}}} =
\frac{ab(-1)}{\sqrt{a^{2} + b^{2} - 2ab\cdot0}} = -\frac{ab}{\sqrt{a^{2} + b^{2}}}
\]

Result:
\[
f'(\frac{\pi}{2}) = \frac{ab}{\sqrt{a^{2} + b^{2}}}
\]

\[
f'(\pi) = 0
\]

\[
f'(\frac{3\pi}{2}) = -\frac{ab}{\sqrt{a^{2} + b^{2}}}
\]

\end{document}
