\documentclass[a4paper, 10pt]{scrartcl}

\usepackage[latin1]{inputenc}

\newcommand*\deriv{\mathrm{d}}
\newcommand*\euler{\mathrm{e}}

\begin{document}

\section{Exercise 1020}

Given:
\[
x = \frac{t - \euler^{-t^{2}}}{2t^{2}}
\]
\[
t\frac{\deriv x}{\deriv t} + 2x = \euler^{-t^{2}} + \frac{1}{2t}
\]

Solution:
\[
\frac{\deriv x}{\deriv t} = \frac{(1 - (-2t)\euler^{-t^{2}})2t^{2} - (t - \euler^{-t^{2}})\cdot 2\cdot 2t}{(2t^{2})^{2}} =
\]
\[
\frac{2t^{2} - (-2t)2t^{2}\euler^{-t^{2}} - (4t^{2} - 4t\euler^{-t^{2}})}{4t^{4}} =
\]
\[
\frac{2t^{2} + 4t^{3}\euler^{-t^{2}} - 4t^{2} + 4t\euler^{-t^{2}}}{4t^{4}} =
\]
\[
\frac{\euler^{-t^{2}}(4t^{3} + 4t) - 2t^{2}}{4t^{4}} = \frac{2t(\euler^{-t^{2}}(2t^{2} + 2) - t)}{4t^{4}} =
\]
\[
\frac{\euler^{-t^{2}}(2t^{2} + 2) - t}{2t^{3}}
\]

\[
\frac{\deriv x}{\deriv t} = \frac{\euler^{-t^{2}}(2t^{2} + 2) - t}{2t^{3}}
\]

\[
x = \frac{t - \euler^{-t^{2}}}{2t^{2}}
\]

\[
t\frac{\deriv x}{\deriv t} + 2x = \euler^{-t^{2}} + \frac{1}{2t}
\]

\[
t\frac{\euler^{-t^{2}}(2t^{2} + 2) - t}{2t^{3}} + 2\frac{t - \euler^{-t^{2}}}{2t^{2}} = \euler^{-t^{2}} + \frac{1}{2t}
\]
\[
\frac{\euler^{-t^{2}}(2t^{2} + 2) - t}{2t^{2}} + \frac{t - \euler^{-t^{2}}}{t^{2}} = \frac{2t\euler^{-t^{2}} + 1}{2t}
\]
\[
\frac{\euler^{-t^{2}}(2t^{2} + 2) - t + 2(t - \euler^{-t^{2}})}{2t^{2}} = \frac{2t\euler^{-t^{2}} + 1}{2t}
\]
\[
\frac{\euler^{-t^{2}}(2t^{2} + 2) - t + 2t - 2\euler^{-t^{2}}}{2t^{2}} = \frac{2t\euler^{-t^{2}} + 1}{2t}
\]
\[
\frac{2t^{2}\euler^{-t^{2}} + 2\euler^{-t^{2}} - t + 2t - 2\euler^{-t^{2}}}{2t^{2}} = \frac{2t\euler^{-t^{2}} + 1}{2t}
\]
\[
\frac{2t^{2}\euler^{-t^{2}} + t}{2t^{2}} = \frac{2t\euler^{-t^{2}} + 1}{2t}
\]
\[
\frac{2t^{2}\euler^{-t^{2}} + t}{2t^{2}} - \frac{2t\euler^{-t^{2}} + 1}{2t} = 0
\]
\[
\frac{2t^{2}\euler^{-t^{2}} + t - t(2t\euler^{-t^{2}} + 1)}{2t^{2}} = 0
\]
\[
\frac{2t^{2}\euler^{-t^{2}} + t - 2t^{2}\euler^{-t^{2}} - t)}{2t^{2}} = 0
\]
\[
\frac{0}{2t^{2}} = 0
\]
\[
0 = 0
\]

\end{document}
