\documentclass[a4paper, 10pt]{scrartcl}

\usepackage[latin1]{inputenc}

\begin{document}

\section{Exercise 881}

Given:
\[
y = \sin^{3}{x} + \cos^{3}{x}
\]

Solution:
\[
y' = 3\sin^{2}{x}\cos{x} + 3\cos^{2}{x}(-\sin{x}) = 3(\sin^{2}{x}\cos{x} - \cos^{2}{x}\sin{x})
\]

Result:
\[
y' = 3(\sin^{2}{x}\cos{x} - \cos^{2}{x}\sin{x})
\]

\section{Exercise 882}

Given:
\[
y = \tan^{3}{x} - 3\tan{x} + 3x
\]

Solution:
\[
y' = 3\tan^{2}{x}\frac{1}{\cos^{2}{x}} - 3\frac{1}{\cos^{2}{x}} + 3 = 3(\frac{\tan^{2}{x}}{\cos^{2}{x}} - \frac{1}{\cos^{2}{x}} + 1) =
\]
\[
3(\frac{\tan^{2}{x} - 1}{\cos^{2}{x}} + 1)
\]

Using $1 + \tan^{2}{x} = \frac{1}{\cos^{2}{x}}$

\[
y' = 3(\frac{\tan^{2}{x} - 1}{\cos^{2}{x}} + 1) = 3((\tan^{2}{x} + 1)(\tan^{2}{x} - 1) + 1) =
\]
\[
3(((\tan^{2}{x})^{2} - 1^{2}) + 1) = 3(\tan^{4}{x} - 1 + 1) = 3\tan^{4}{x}
\]

Result:
\[
y' = 3\tan^{4}{x}
\]

\end{document}
