\documentclass[a4paper, 10pt]{scrartcl}

\usepackage[latin1]{inputenc}

\begin{document}

\section{Exercise 1}

Given:
\[f(x) = x^{n}\cos{ax}\ln{x}\]

Solution:
\[u(x) = x^{n}\cos{ax}\]
\[u_{0}(x) = x^{n}\]
\[u'_{0}(x) = nx^{n - 1}\]
\[v_{0}(x) = \cos{ax}\]
\[v'_{0}(x) = a(-\sin{ax}) = -a\sin{ax}\]
\[u'(x) = x^{n}(-a\sin{ax}) + nx^{n - 1}\cos{ax}\]
\[u'(x) = -ax^{n}\sin{ax} + nx^{n - 1}\cos{ax}\]
\[u'(x) = x^{n - 1}(-ax\sin{ax} + n\cos{ax})\]
\[u'(x) = x^{n - 1}(-ax\sin{ax} + n\cos{ax}) = x^{n - 1}(n\cos{ax} - ax\sin{ax})\]

\[v(x) = \ln{x}\]
\[v'(x) = \frac{1}{x}\]

\[f'(x) = x^{n}\cos{ax}\frac{1}{x} + x^{n - 1}(n\cos{ax} - ax\sin{ax})\ln{x}\]
\[f'(x) = x^{n - 1}\cos{ax} + x^{n - 1}(n\cos{ax} - ax\sin{ax})\ln{x}\]
\[f'(x) = x^{n - 1}(\cos{ax} + (n\cos{ax} - ax\sin{ax})\ln{x})\]
\[f'(x) = x^{n - 1}(\cos{ax} + n\cos{ax}\ln{x} - ax\sin{ax}\ln{x})\]

Result:
\[f'(x) = x^{n - 1}(\cos{ax} + n\cos{ax}\ln{x} - ax\sin{ax}\ln{x})\]

\end{document}
