\documentclass[a4paper, 10pt]{scrartcl}

\usepackage[latin1]{inputenc}

\newcommand*\euler{\mathrm{e}}

\begin{document}

\section{Exercise 1049}

Given:
\[
\euler^{xy} - x^{2} + y^{3} = 0
\]

Solution:
\[
(xy)'\euler^{xy} - 2x + 3y^{2}y' = 0
\]
\[
(y + xy')\euler^{xy} - 2x + 3y^{2}y' = 0
\]
\[
y\euler^{xy} + xy'\euler^{xy} - 2x + 3y^{2}y' = 0
\]
\[
y\euler^{xy} + y'(x\euler^{xy} + 3y^{2}) - 2x = 0
\]
\[
y'(x\euler^{xy} + 3y^{2}) = 2x - y\euler^{xy}
\]
\[
y' = \frac{2x - y\euler^{xy}}{x\euler^{xy} + 3y^{2}}
\]

\[
y'(0) = \frac{2\cdot 0 - y(0)\euler^{0\cdot y(0)}}{0\euler^{0\cdot y(0)} + 3y(0)^{2}}
\]
\[
y'(0) = \frac{-y(0)}{3y(0)^{2}}
\]

Computing $y(0)$:
\[
\euler^{xy} - x^{2} + y^{3} = 0
\]
\[
\euler^{0\cdot y(0)} - 0^{2} + y(0)^{3} = 0
\]
\[
1 + y(0)^{3} = 0
\]
\[
y(0)^{3} = -1
\]
\[
y(0) = \sqrt[3]{-1} = -1
\]

\[
y'(0) = \frac{-1}{3y(0)} = \frac{-1}{3\cdot(-1)} = \frac{1}{3}
\]

Result:
\[
y'(0) = \frac{1}{3}
\]

\end{document}
