\documentclass[a4paper, 10pt]{scrartcl}

\usepackage[latin1]{inputenc}

\begin{document}

\section{Exercise 66.8}

\[2\sin{2\phi}\sin{\phi} = \cos{\phi}\]

Using:
\[\sin{\alpha}\sin{\beta} = -\frac{1}{2}(\cos{(\alpha + \beta)} - \cos{(\alpha - \beta)})\]

\[2\left(-\frac{1}{2}(\cos{(2\phi + \phi)} - \cos{(2\phi - \phi)})\right) = \cos{\phi}\]
\[-(\cos{(2\phi + \phi)} - \cos{(2\phi - \phi)}) = \cos{\phi}\]
\[-(\cos{3\phi} - \cos{\phi}) = \cos{\phi}\]
\[\cos{\phi} - \cos{3\phi} = \cos{\phi}\]
\[\cos{\phi} - \cos{3\phi} - \cos{\phi} = 0\]
\[-\cos{3\phi} = 0\]
\[\cos{3\phi} = 0\]
\[3\phi = \arccos{0}\]
\[3\phi = \frac{\pi}{2}\]
\[\phi = \frac{\pi}{6}\]

Result:
$2\sin{2\phi}\sin{\phi} = \cos{\phi}$ for $\phi = \frac{\pi}{6}$

\end{document}
