\documentclass[a4paper, 10pt]{scrartcl}

\usepackage[latin1]{inputenc}

\begin{document}

\section{Exercise 855a}

Given:
\[
y = \frac{1}{2x^{2}} - \frac{1}{3x^{3}}
\]

Solution:
\[
y = \frac{1}{2x^{2}} - \frac{1}{3x^{3}} = \frac{1}{2}x^{-2} - \frac{1}{3}x^{-3}
\]

\[
y' = \frac{1}{2}\cdot(-2)x^{-2 - 1} - \frac{1}{3}\cdot(-3)x^{-3 - 1} = -x^{-3} + x^{-4} =
\]
\[
x^{-4} - x^{-3} = \frac{1}{x^{4}} - \frac{1}{x^{3}} = \frac{1 - x}{x^{4}}
\]

Result:
\[
y' = \frac{1 - x}{x^{4}}
\]

\section{Exercise 855b}

Given:
\[
y = \frac{8}{\sqrt[4]{x}} - \frac{6}{\sqrt[3]{x}}
\]

Solution:
\[
y = 8x^{-\frac{1}{4}} - 6x^{-\frac{1}{3}}
\]

\[
y' = 8\cdot(-\frac{1}{4})x^{-\frac{1}{4} - 1} - 6\cdot(-\frac{1}{3})x^{-\frac{1}{3} - 1} =
\]
\[
-2x^{-\frac{5}{4}} + 2x^{-\frac{4}{3}} = 2x^{-\frac{4}{3}} - 2x^{-\frac{5}{4}} =
\]
\[
2\left(x^{-\frac{4}{3}} - x^{-\frac{5}{4}}\right) = 2\left(\frac{1}{\sqrt[3]{x^{4}}} - \frac{1}{\sqrt[4]{x^{5}}}\right) =
\]
\[
2\left(\frac{1}{x\sqrt[3]{x}} - \frac{1}{x\sqrt[4]{x}}\right) = \frac{2}{x}\left(\frac{1}{\sqrt[3]{x}} - \frac{1}{\sqrt[4]{x}}\right)
\]

Result:
\[
y' = \frac{2}{x}\left(\frac{1}{\sqrt[3]{x}} - \frac{1}{\sqrt[4]{x}}\right)
\]

\end{document}
