\documentclass[a4paper, 10pt]{scrartcl}

\usepackage[latin1]{inputenc}

\begin{document}

\section{Exercise 66.5}

\[f(x) = 3\sin{\frac{\pi}{3}}\cos{\frac{\pi}{6}}\]

Using:
\[\sin{\alpha}\cos{\beta} = \frac{1}{2}(\sin{(\alpha + \beta)} + \sin{(\alpha - \beta)})\]

\[f(x) = 3\left(\frac{1}{2}(\sin{(\frac{\pi}{3} + \frac{\pi}{6})} +
        \sin{(\frac{\pi}{3} - \frac{\pi}{6})})\right)\]

Using:
\[\frac{\pi}{3} + \frac{\pi}{6} = \frac{2\pi + \pi}{6} = \frac{3\pi}{6} = \frac{\pi}{2}\]

\[f(x) = 3\left(\frac{1}{2}(\sin{\frac{\pi}{2}} +
        \sin{(\frac{\pi}{3} - \frac{\pi}{6})})\right)\]

Using:
\[\frac{\pi}{3} - \frac{\pi}{6} = \frac{2\pi - \pi}{6} = \frac{\pi}{6}\]

\[f(x) = 3\left(\frac{1}{2}(\sin{\frac{\pi}{2}} +
        \sin{\frac{\pi}{6}})\right)\]

\[f(x) = \frac{3}{2}(\sin{\frac{\pi}{2}} + \sin{\frac{\pi}{6}})\]

Result:
\[f(x) = 3\sin{\frac{\pi}{3}}\cos{\frac{\pi}{6}}
       = \frac{3}{2}(\sin{\frac{\pi}{2}} + \sin{\frac{\pi}{6}})\]

\end{document}
