\documentclass[a4paper, 10pt]{scrartcl}

\usepackage[latin1]{inputenc}

\begin{document}

\section{Exercise 64.4}

Given:
\[-3\sin{\omega t} - 6\cos{\omega t} = R\sin{(\omega t + \alpha)}\]

Using:
\[\sin{(\alpha + \beta)} = \sin{\alpha}\cos{\beta} + \cos{\alpha}\sin{\beta}\]

Computation of $R$:
\[R\sin{(\omega t + \alpha)} =
R(\sin{\omega t}\cos{\alpha} + \cos{\omega t}\sin{\alpha})\]
\[R\sin{\omega t}\cos{\alpha} + R\cos{\omega t}\sin{\alpha}\]
\[R\cos{\alpha}\sin{\omega t} + R\sin{\alpha}\cos{\omega t}\]

\[R\cos{\alpha} = -3\]
\[\cos{\alpha} = \frac{-3}{R}\]

\[R\sin{\alpha} = -6\]
\[\sin{\alpha} = \frac{-6}{R}\]

\[\sin^{2}{\alpha} + \cos^{2}{\alpha} = 1\]
\[\left(\frac{-6}{R}\right)^{2} + \left(\frac{-3}{R}\right)^{2} = 1\]
\[\frac{(-6)^{2}}{R^{2}} + \frac{(-3)^{2}}{R^{2}} = 1\]
\[(-6)^{2} + (-3)^{2} = R^{2}\]
\[R = \sqrt{(-6)^{2} + (-3)^{2}} \approx 6,708\]

Computation of $\alpha$:

Result:

\end{document}
