\documentclass[a4paper, 10pt]{scrartcl}

\usepackage[latin1]{inputenc}

\begin{document}

\section{Exercise 777}

Given:
\[
\lim_{x\to 0}{\frac{1 - \cos{mx}}{x^{2}}}
\]

Solution:
\[
u(x) = 1 - \cos{mx}
\]
\[
u'(x) = 0 - (-m\sin{mx}) = m\sin{mx}
\]
\[
u'(0) = m\sin{m\cdot 0} = m\sin{0} = m\cdot 0 = 0
\]

\[
v(x) = x^{2}
\]
\[
v'(x) = 2x^{2 - 1} = 2x^{1} = 2x
\]
\[
v'(0) = 2\cdot 0 = 0
\]

\[
u'(x) = m\sin{mx}
\]
\[
u''(x) = m(m\cos{mx}) = m^{2}\cos{mx}
\]
\[
u''(0) = m^{2}\cos{m\cdot 0} = m^{2}
\]

\[
v'(x) = 2x
\]
\[
v''(x) = 2
\]
\[
v''(0) = 2
\]

\[
\lim_{x\to 0}{\frac{1 - \cos{mx}}{x^{2}}} = \lim_{x\to 0}{\frac{u'(x)}{v'(x)}} = \lim_{x\to 0}{\frac{u''(x)}{v''(x)}}
= \frac{m^{2}}{2}
\]

Result:
\[
\lim_{x\to 0}{\frac{1 - \cos{mx}}{x^{2}}} = \frac{m^{2}}{2}
\]

\section{Exercise 778}

Given:
\[
\lim_{x\to 0}{\frac{1 - \cos{2x} + \tan^{2}{x}}{x\sin{x}}}
\]

Solution:
\[
u(x) = 1 - \cos{2x} + \tan^{2}{x}
\]
\[
u'(x) = 0 - (-2\sin{2x}) + 2\tan{x}(\frac{1}{\cos^{2}{x}}) = 2\sin{2x} + \frac{2\tan{x}}{\cos^{2}{x}} =
\]
\[
2\sin{2x} + \frac{2\frac{\sin{x}}{\cos{x}}}{\cos^{2}{x}} = 2\sin{2x} + \frac{2\sin{x}}{\cos^{3}{x}}
\]
\[
u'(0) = 2\sin{2\cdot 0} + \frac{2\sin{0}}{\cos^{3}{0}} = 2\cdot 0 + \frac{2\cdot 0}{1^{3}} = 0
\]

\[
v(x) = x\sin{x}
\]
\[
v'(x) = \sin{x} + x\cos{x}
\]
\[
v'(0) = \sin{0} + 0\cos{0} = 0
\]

\[
u'(x) = 2\sin{2x} + \frac{2\sin{x}}{\cos^{3}{x}}
\]
\[
u''(x) = 2\cdot 2\cos{2x} + 2\frac{\cos{x}\cos^{3}{x} - \sin{x}3\cos^{2}{x}(-\sin{x})}{(\cos^{3}{x})^{2}} =
\]
\[
4\cos{2x} + 2\frac{\cos^{4}{x} + 3\sin^{2}{x}\cos^{2}{x}}{\cos^{6}{x}}
\]
\[
u''(0) = 4\cos{2\cdot 0} + 2\frac{\cos^{4}{0} + 3\sin^{2}{0}\cos^{2}{0}}{\cos^{6}{0}} = 4 + 2\frac{1 + 3\cdot 0\cdot 1}{1} = 4 + 2 = 6
\]

\[
v'(x) = \sin{x} + x\cos{x}
\]
\[
v''(x) = \cos{x} + \cos{x} + x(-\sin{x}) = 2\cos{x} - \sin{x}
\]
\[
v''(0) = 2\cos{0} - \sin{0} = 2
\]

\[
\lim_{x\to 0}{\frac{1 - \cos{2x} + \tan^{2}{x}}{x\sin{x}}} = \lim_{x\to 0}{\frac{u'(x)}{v'{x}}} = \lim_{x\to 0}{\frac{u''(x)}{v''{x}}} =
\frac{6}{3} = 3
\]

Result:
\[
\lim_{x\to 0}{\frac{1 - \cos{2x} + \tan^{2}{x}}{x\sin{x}}} = 3
\]

\end{document}
