\documentclass[a4paper, 10pt]{scrartcl}

\usepackage[latin1]{inputenc}

\begin{document}

\section{Exercise 1013}

Given:
\[
f(x) = (x^{2} + a^{2})\arctan{\frac{x}{a}} - ax
\]

Solution:
\[
f'(x) = 2x\arctan{\frac{x}{a}} + (x^{2} + a^{2})\frac{1}{1 + (\frac{x}{a})^{2}}\frac{1}{a} - a =
\]
\[
2x\arctan{\frac{x}{a}} + \frac{x^{2} + a^{2}}{1 + \frac{x^{2}}{a^{2}}}\frac{1}{a} - a =
\]
\[
2x\arctan{\frac{x}{a}} + \frac{x^{2} + a^{2}}{\frac{a^{2} + x^{2}}{a^{2}}}\frac{1}{a} - a =
\]
\[
2x\arctan{\frac{x}{a}} + \frac{a^{2}(x^{2} + a^{2})}{a^{2} + x^{2}}\frac{1}{a} - a =
\]
\[
2x\arctan{\frac{x}{a}} + \frac{a^{2}}{1}\frac{1}{a} - a = 2x\arctan{\frac{x}{a}} + a - a = 2x\arctan{\frac{x}{a}}
\]

\[
f'(x) = 2x\arctan{\frac{x}{a}}
\]

\[
f'(a) = 2a\arctan{\frac{a}{a}} = 2a\arctan{1} = 2a\frac{\pi}{4} = \frac{a\pi}{2}
\]

Result:
\[
f'(a) = \frac{a\pi}{2}
\]

\end{document}
