\documentclass[a4paper, 10pt]{scrartcl}

\usepackage[latin1]{inputenc}

\newcommand*\euler{\mathrm{e}}

\begin{document}

\section{Exercise 1016}

Given:
\[
f(u) = \euler^{-\frac{u}{a}}\cos{\frac{u}{a}}
\]

Solution:
\[
\left(\euler^{-\frac{u}{a}}\right)' = -\frac{1}{a}\euler^{\frac{u}{a}}
\]
\[
(\cos{\frac{u}{a}})' = (-\sin{\frac{u}{a}})\frac{1}{a} = -\frac{\sin{\frac{u}{a}}}{a}
\]

\[
f'(u) = -\frac{1}{a}\euler^{\frac{u}{a}}\cos{\frac{u}{a}} + \euler^{-\frac{u}{a}}(-\frac{\sin{\frac{u}{a}}}{a}) =
-\frac{1}{a}\euler^{\frac{u}{a}}(\cos{\frac{u}{a}} + \sin{\frac{u}{a}})
\]

\[
f'(u) = -\frac{1}{a}\euler^{\frac{u}{a}}(\cos{\frac{u}{a}} + \sin{\frac{u}{a}})
\]

\[
f(0) = \euler^{-\frac{0}{a}}\cos{\frac{0}{a}} = \euler^{0}\cos{0} = 1\cdot 1 = 1
\]

\[
f'(0) = -\frac{1}{a}\euler^{\frac{0}{a}}(\cos{\frac{0}{a}} + \sin{\frac{0}{a}}) = -\frac{1}{a}\euler^{0}(\cos{0} + \sin{0}) =
-\frac{1}{a}\cdot 1 \cdot(1 + 0) = -\frac{1}{a}
\]

\[
f(0) + af'(0) = 1 + a\cdot\frac{-1}{a} = 1 + (-1) = 1 - 1 = 0
\]

Result:
\[
f(0) + af'(0) = 0
\]

\end{document}
