\documentclass[a4paper, 10pt]{scrartcl}

\usepackage[latin1]{inputenc}

\begin{document}

\section{Exercise 885}

Given:
\[
y = \sqrt{1 + \sin{2x}} - \sqrt{1 - \sin{2x}}
\]

Solution:
\[
y' = \frac{0 + 2\cos{2x}}{2\sqrt{1 + \sin{2x}}} - \frac{0 - 2\cos{2x}}{2\sqrt{1 - \sin{2x}}} =
\]
\[
\frac{\cos{2x}}{\sqrt{1 + \sin{2x}}} - \frac{\cos{2x}}{\sqrt{1 - \sin{2x}}} =
\]
\[
\cos{2x}\left(\frac{1}{\sqrt{1 + \sin{2x}}} - \frac{1}{\sqrt{1 - \sin{2x}}}\right) =
\]
\[
\cos{2x}\left(\frac{\sqrt{1 - \sin{2x}} - \sqrt{1 + \sin{2x}}}{\sqrt{1 + \sin{2x}}\sqrt{1 - \sin{2x}}}\right) =
\]
\[
\cos{2x}\left(\frac{\sqrt{1 - \sin{2x}} - \sqrt{1 + \sin{2x}}}{\sqrt{(1 + \sin{2x})(1 - \sin{2x})}}\right) =
\]
\[
\cos{2x}\left(\frac{\sqrt{1 - \sin{2x}} - \sqrt{1 + \sin{2x}}}{\sqrt{1^{2} - \sin^{2}{2x}}}\right) =
\]
\[
\cos{2x}\left(\frac{\sqrt{1 - \sin{2x}} - \sqrt{1 + \sin{2x}}}{\sqrt{\cos^{2}{2x}}}\right) =
\]
\[
\cos{2x}\left(\frac{\sqrt{1 - \sin{2x}} - \sqrt{1 + \sin{2x}}}{\pm\cos{2x}}\right) =
\]
\[
\pm(\sqrt{1 - \sin{2x}} - \sqrt{1 + \sin{2x}})
\]

Result:
\[
y' = \pm(\sqrt{1 - \sin{2x}} - \sqrt{1 + \sin{2x}})
\]

\end{document}
