\documentclass[a4paper, 10pt]{scrartcl}

\usepackage[latin1]{inputenc}

\begin{document}

\section{$\cos{jx}$}

Given:
\[\cos{x} = \frac{1}{2}(e^{jx} + e^{-jx})\]

Solution:
\[\cos{jx} = \frac{1}{2}(e^{j(jx)} + e^{-j(jx)}) =
             \frac{1}{2}(e^{jjx} + e^{-jjx})\]

\[\cos{jx} = \frac{1}{2}(e^{-1\cdot x} + e^{-(-1)x}) =
             \frac{1}{2}(e^{-x} + e^{x}) = \frac{1}{2}(e^{x} + e^{-x})\]

\[\cosh{x} = \frac{1}{2}(e^{x} + e^{-x}) = \cos{jx}\]

Result:
\[\cos{jx} = \cosh{x}\]

\section{$\sin{jx}$}

Given:
\[\sin{x} = \frac{1}{2j}(e^{jx} - e^{-jx})\]

Solution:
\[\sin{jx} = \frac{1}{2j}(e^{j(jx)} - e^{-j(jx)}) = \frac{1}{2j}(e^{jjx} - e^{-jjx})\]
\[\sin{jx} = \frac{1}{2j}(e^{jjx} - e^{-jjx}) = \frac{1}{2j}(e^{-1\cdot x} - e^{-(-1)x})\]
\[\sin{jx} = \frac{1}{2j}(e^{-1\cdot x} - e^{-(-1)x}) = \frac{1}{2j}(e^{-x} - e^{x})\]
\[\sin{jx} = \frac{1}{2j}(e^{-x} - e^{x}) = -\frac{1}{2j}(e^{x} - e^{-x})\]

\[\sinh{x} = \frac{1}{2}(e^{x} - e^{-x})\]

\[\sin{jx} = -\frac{1}{j}\sinh{x} = -\frac{1}{j}\frac{j}{j}\sinh{x} = -\frac{j}{jj}\sinh{x}\]
\[\sin{jx} = -\frac{j}{-1}\sinh{x} = j\sinh{x}\]

Result:
\[\sin{jx} = j\sinh{x}\]

\end{document}
