\documentclass[a4paper, 10pt]{scrartcl}

\usepackage[latin1]{inputenc}

\newcommand*\euler{\mathrm{e}}

\begin{document}

\section{Exercise 1023a}

Given:
\[
y = x\ln{x}
\]

Solution:
\[
y' = \ln{x} + x\frac{1}{x} = \ln{x} + 1
\]
\[
y'' = \frac{1}{x} = x^{-1}
\]
\[
y''' = (-1)x^{-1 - 1} = -x^{-2} = -\frac{1}{x^{2}}
\]

Result:
\[
y''' = -\frac{1}{x^{2}}
\]

\section{Exercise 1023b}

Given:
\[
s = t\euler^{-t}
\]

Solution:
\[
s' = \euler^{-t} + t(-1)\euler^{-t} = \euler^{-t}(1 - t)
\]
\[
s'' = (-1)\euler^{-t}(1 - t) + \euler^{-t}(-1) = \euler^{-t}((-1)(1 - t) + (-1)) = \euler^{-t}(-1 + t - 1) = \euler^{-t}(t - 2)
\]
\[
s''' = (-1)\euler^{-t}(t - 2) + \euler^{-t} = \euler^{-t}((-1)(t - 2) + 1) = \euler^{-t}(-t + 2 + 1) = \euler^{-t}(3 - t)
\]

Result:
\[
s''' = \euler^{-t}(3 - t)
\]

\section{Exercise 1023c}

Given:
\[
y = \arctan{\frac{x}{a}}
\]

Solution:
\[
y' = \frac{\frac{1}{a}}{1 + \left(\frac{x}{a}\right)^{2}} = \frac{\frac{1}{a}}{1 + \frac{x^{2}}{a^{2}}} =
\frac{\frac{1}{a}}{\frac{a^{2} + x^{2}}{a^{2}}} =
\]
\[
\frac{\frac{1}{a}a^{2}}{a^{2} + x^{2}} = \frac{a}{a^{2} + x^{2}}
\]

Result 1: $y' = \frac{a}{a^{2} + x^{2}}$\\

\[
y'' = \frac{0(a^{2} + x^{2}) - a2x}{(a^{2} + x^{2})^{2}} = \frac{-2ax}{(a^{2} + x^{2})^{2}}
\]

Result 2: $y'' = \frac{-2ax}{(a^{2} + x^{2})^{2}}$\\

\[
y''' = \frac{-2a(a^{2} + x^{2})^{2} - (-2ax)2(a^{2} + x^{2})2x}{(a^{2} + x^{2})^{4}} =
\]
\[
\frac{(a^{2} + x^{2})(-2a(a^{2} + x^{2}) + 8ax^{2})}{(a^{2} + x^{2})^{4}} = \frac{-2a^{3} - 2ax^{2} + 8ax^{2}}{(a^{2} + x^{2})^{3}} =
\]
\[
\frac{-2a^{3} + 6ax^{2}}{(a^{2} + x^{2})^{3}} = \frac{2a(3x^{2} - a^{2})}{(a^{2} + x^{2})^{3}}
\]

Result:
\[
y''' = \frac{2a(3x^{2} - a^{2})}{(a^{2} + x^{2})^{3}}
\]

\end{document}
