\documentclass[a4paper, 10pt]{scrartcl}

\usepackage[latin1]{inputenc}

\newcommand*\euler{\mathrm{e}}

\begin{document}

\section{Exercise 957}

Given:
\[
y = \ln{\frac{\euler^{x}}{x^{2} + 1}}
\]

Solution:
\[
y' = \frac{1}{\frac{\euler^{x}}{x^{2} + 1}}\cdot\frac{\euler^{x}(x^{2} + 1) - \euler^{x}(2x + 0)}{(x^{2} + 1)^{2}} =
\]
\[
\frac{x^{2} + 1}{\euler^{x}}\cdot\frac{\euler^{x}x^{2} + \euler^{x} - 2x\euler^{x}}{(x^{2} + 1)^{2}} =
\]
\[
\frac{1}{\euler^{x}}\cdot\frac{\euler^{x}(x^{2} + 1 - 2x)}{x^{2} + 1} =
\]
\[
\frac{1}{1}\cdot\frac{x^{2} + 1 - 2x}{x^{2} + 1} = \frac{(x - 1)^{2}}{x^{2} + 1}
\]

Result:
\[
y' = \frac{(x - 1)^{2}}{x^{2} + 1}
\]

\end{document}
