\documentclass[a4paper, 10pt]{scrartcl}

\usepackage[latin1]{inputenc}

\begin{document}

\section{Exercise 947a}

Given:
\[
y = \frac{\cos{x}}{\sin^{2}{x}} + \ln{\tan{\frac{x}{2}}}
\]

Solution:
\[
y' = \frac{(-\sin{x})\sin^{2}{x} - \cos{x}\cdot 2\sin{x}\cos{x}}{(\sin^{2}{x})^{2}} +
    \frac{1}{\tan{\frac{x}{2}}}\frac{1}{\cos^{2}{\frac{x}{2}}}\frac{1}{2}
\]

\[
y' = \frac{-\sin^{3}{x} - 2\cos^{2}{x}\sin{x}}{\sin^{4}{x}} +
    \frac{1}{2}\frac{\cos{\frac{x}{2}}}{\sin{\frac{x}{2}}}\frac{1}{\cos^{2}{\frac{x}{2}}}
\]

\[
y' = -\frac{1}{\sin{x}} - 2\frac{\cos^{2}{x}}{\sin^{3}{x}} +
    \frac{1}{2}\frac{1}{\sin{\frac{x}{2}}}\frac{1}{\cos{\frac{x}{2}}}
\]

\[
y' = -\frac{1}{\sin{x}} - 2\frac{\cos^{2}{x}}{\sin^{3}{x}} +
    \frac{1}{\sin{x}} = -2\frac{\cos^{2}{x}}{\sin^{3}{x}} = -2\frac{\cot^{2}{x}}{\sin{x}}
\]

Result:
\[
y' = -2\frac{\cot^{2}{x}}{\sin{x}}
\]

\section{Exercise 947b}

Given:
\[
y = \ln{\frac{x^{2}}{\sqrt{1 - ax^{4}}}}
\]

Solution:
\[
y' = \frac{1}{\frac{x^{2}}{\sqrt{1 - ax^{4}}}}\frac{2x\sqrt{1 - ax^{4}} - x^{2}\frac{1}{2\sqrt{1 - ax^{4}}}(0 - 4ax^{3})}{(\sqrt{1 - ax^{4}})^{2}} =
\]
\[
\frac{\sqrt{1 - ax^{4}}}{x^{2}}\frac{2x\sqrt{1 - ax^{4}} + \frac{2ax^{5}}{\sqrt{1 - ax^{4}}}}{(\sqrt{1 - ax^{4}})^{2}} =
\]
\[
\frac{1}{x^{2}}\frac{2x\sqrt{1 - ax^{4}} + \frac{2ax^{5}}{\sqrt{1 - ax^{4}}}}{\sqrt{1 - ax^{4}}} =
\]
\[
\frac{1}{x^{2}}\left(2x + \frac{2ax^{5}}{\sqrt{1 - ax^{4}}\sqrt{1 - ax^{4}}}\right) =
\]
\[
\frac{2}{x} + \frac{2ax^{3}}{1 - ax^{4}} = \frac{2(1 - ax^{4}) + 2ax^{4}}{x(1 - ax^{4})} = \frac{2 - 2ax^{4} + 2ax^{4}}{x(1 - ax^{4})} =
\]
\[
\frac{2}{x(1 - ax^{4})} = \frac{2}{x - ax^{5}}
\]

Result:
\[
y' = \frac{2}{x - ax^{5}}
\]

\end{document}
