\documentclass[a4paper, 10pt]{scrartcl}

\usepackage[latin1]{inputenc}

\newcommand*\euler{\mathrm{e}}

\begin{document}

\section{Exercise 987a}

Given:
\[
y = x\sqrt{1 - x^{2}} + \arcsin{x}
\]

Solution:
\[
y' = \sqrt{1 - x^{2}} + x\cdot\frac{1}{2\sqrt{1 - x^{2}}}\cdot(0 - 2x) + \frac{1}{\sqrt{1 - x^{2}}} =
\]
\[
\sqrt{1 - x^{2}} + \frac{-x^{2}}{\sqrt{1 - x^{2}}} + \frac{1}{\sqrt{1 - x^{2}}} =
\]
\[
\sqrt{1 - x^{2}} + \frac{1 -x^{2}}{\sqrt{1 - x^{2}}} = \sqrt{1 - x^{2}} + \sqrt{1 - x^{2}} = 2\sqrt{1 - x^{2}}
\]

Result:
\[
y' = 2\sqrt{1 - x^{2}}
\]

\section{Exercise 987b}

Given:
\[
y = \arcsin{\euler^{3x}}
\]

Solution:

Result:

\end{document}
