\documentclass[a4paper, 10pt]{scrartcl}

\usepackage[latin1]{inputenc}

\begin{document}

\section{Exercise 68.6a}

Given:
\[f(x) = 4\ln{9x}\]

Solution:
\[f'(x) = 4\frac{1}{x} = \frac{4}{x}\]

Result:
\[f'(x) = \frac{4}{x}\]

\section{Exercise 68.6b}

Given:
\[f(x) = \frac{e^{x} - e^{-x}}{2}\]

Solution:
\[f'(x) = \frac{1}{2}(e^{x} - (-1)e^{-x}) = \frac{1}{2}(e^{x} + e^{-x})\]

Result:
\[f'(x) = \frac{1}{2}(e^{x} + e^{-x})\]

\section{Exercise 68.6c}

Given:
\[f(x) = \frac{1 - \sqrt{x}}{x}\]

Solution:
\[f(x) = \frac{1 - \sqrt{x}}{x} = \frac{1}{x} - \frac{\sqrt{x}}{x}\]
\[f(x) = \frac{1}{x} - \frac{\sqrt{x}}{x} = x^{-1} - x^{\sqrt{1}{2} - 1} =
         x^{-1} - x^{-\sqrt{1}{2}}\]

\[f'(x) = -1x^{-1 - 1} - (-\frac{1}{2})x^{-\frac{1}{2} - 1} =
          -x^{-2} + \frac{1}{2}x^{-\frac{3}{2}}\]

\[f'(x) = -x^{-2} + \frac{1}{2}x^{-\frac{3}{2}} =
           -\frac{1}{x^{2}} + \frac{1}{2}\cdot\frac{1}{x^{\frac{3}{2}}\]

\[f'(x) = -\frac{1}{x^{2}} + \frac{1}{2\sqrt{x^{3}} = \frac{1}{2\sqrt{x^{3}} - \frac{1}{x^{2}}\]

Result:
\[f'(x) = \frac{1}{2\sqrt{x^{3}} - \frac{1}{x^{2}}\]

\end{document}
