\documentclass[a4paper, 10pt]{scrartcl}

\usepackage[latin1]{inputenc}

\begin{document}

\section{Exercise 900}

Given:
\[
y = \frac{1 + \sin{2x}}{1 - \sin{2x}}
\]

Solution:
\[
y = (1 + \sin{2x})(1 - \sin{2x})^{-1}
\]

\[
y' = (0 + 2\cos{2x})(1 - \sin{2x})^{-1} + (1 + \sin{2x})(-1)(1 - \sin{2x})^{-1 - 1}(0 - 2\cos{2x}) =
\]
\[
2\cos{2x}(1 - \sin{2x})^{-1} + (1 + \sin{2x})(1 - \sin{2x})^{-2}2\cos{2x} =
\]
\[
\frac{2\cos{2x}}{1 - \sin{2x}} + \frac{2\cos{2x}(1 + \sin{2x})}{(1 - \sin{2x})^{2}} =
\]
\[
\frac{2\cos{2x}(1 - \sin{2x}) + 2\cos{2x}(1 + \sin{2x})}{(1 - \sin{2x})^{2}} =
\]
\[
\frac{2\cos{2x}((1 - \sin{2x}) + (1 + \sin{2x}))}{(1 - \sin{2x})^{2}} =
\]
\[
\frac{2\cos{2x}(1 - \sin{2x} + 1 + \sin{2x})}{(1 - \sin{2x})^{2}} =
\]
\[
\frac{2\cos{2x}(2)}{(1 - \sin{2x})^{2}} = \frac{4\cos{2x}}{(1 - \sin{2x})^{2}}
\]

Result:
\[
y' = \frac{4\cos{2x}}{(1 - \sin{2x})^{2}}
\]

\end{document}
