\documentclass[a4paper, 10pt]{scrartcl}

\usepackage[latin1]{inputenc}

\begin{document}

\section{Exercise 607}

Given:
\[
\left|
    \begin{array}{ccc}
    ax & a^{2} + x^{2} & 1\\
    ay & a^{2} + y^{2} & 1\\
    az & a^{2} + z^{2} & 1
    \end{array}
\right|
\]

Solution:
\[
ax(a^{2} + y^{2})1 = a^{3}x + axy^{2}
\]
\[
(a^{2} + x^{2})az\cdot1 = a^{3}z + ax^{2}z
\]
\[
1\cdot ay(a^{2} + z^{2}) = a^{3}y + ayz^{2}
\]
\[
az(a^{2} + y^{2})1 = a^{3}z + ay{2}z
\]
\[
(a^{2} + z^{2})\cdot 1 ax = a^{3}x + axz^{2}
\]
\[
1ay(a^{2} + x^{2}) = a^{3}y + ax^{2}y
\]
\\
\\
\[
a^{3}x + axy^{2} + a^{3}z + ax^{2}z + a^{3}y + ayz^{2} -
\]
\[
(a^{3}z + ay{2}z + a^{3}x + axz^{2} + a^{3}y + ax^{2}y)
\]
\\
\\
\[
a^{3}x + axy^{2} + a^{3}z + ax^{2}z + a^{3}y + ayz^{2} -
\]
\[
a^{3}z - ay{2}z - a^{3}x - axz^{2} - a^{3}y - ax^{2}y
\]
\\
\\
\[
axy^{2} + ax^{2}z + ayz^{2} - ay{2}z - axz^{2} - ax^{2}y =
\]
\[
a(x - z)(y - z)(y - x)
\]

Probe:
\[
a(x - z)(y - z)(y - x) =
\]
\[
a(xy - xz - yz + z^{2})(y - x) =
\]
\[
a(xy^{2} - xyz - y^{2}z + yz^{2} - x^{2}y + x^{2}z + xyz - xz^{2}) =
\]
\[
a(xy^{2} - y^{2}z + yz^{2} - x^{2}y + x^{2}z - xz^{2})
\]

Result:
\[
\left|
    \begin{array}{ccc}
    ax & a^{2} + x^{2} & 1\\
    ay & a^{2} + y^{2} & 1\\
    az & a^{2} + z^{2} & 1
    \end{array}
\right| = a(x - z)(y - z)(y - x)
\]

\end{document}
