\documentclass[a4paper, 10pt]{scrartcl}

\usepackage[latin1]{inputenc}

\begin{document}

\section{Exercise 36.7}

Given:
\[\lim_{x\to 0}{\frac{\sinh{x} - \sin{x}}{x^{3}}}\]

Solution:
\[u(x) = \sinh{x} - \sin{x}\]
\[u(0) = \sinh{0} - \sin{0}\]
\[\sinh{x} = \frac{1}{2}(e^{x} - e^{-x})\]
\[u(0) = \frac{1}{2}(e^{0} - e^{-0}) - \sin{0} = \frac{1}{2}(0 - 0) - 0 = 0\]

\[v(x) = x^{3}\]
\[v(0) = 0^{3} = 0\]

\[u'(x) = \cosh{x} - \cos{x}\]
\[u'(0) = \cosh{0} - \cos{0}\]
\[\cosh{x} = \frac{1}{2}(e^{x} + e^{-x})\]
\[u'(0) = \frac{1}{2}(e^{0} + e^{-0}) - \cos{0} = \frac{1}{2}(1 + 1) - 1 = \frac{1}{2}2 - 1 = 0\]

\[v'(x) = 3x^{3 - 1} = 3x^{2}\]
\[v'(0) = 3\cdot 0^{2} = 3\cdot 0 = 0\]

\[u''(x) = \sinh{x} - (-\sin{x}) = \sinh{x} + \sin{x}\]
\[u''(0) = \sinh{0} + \sin{0} = \frac{1}{2}(e^{0} - e^{-0}) + 0 = \frac{1}{2}(0 - 0) + 0 = 0\]

\[v''(x) = 3\cdot 2x^{2 - 1} = 6x^{1} = 6x\]
\[v''(0) = 6\cdot 0 = 0\]

\[u'''(x) = \cosh{x} + \cos{x}\]
\[u'''(0) = \cosh{0} + \cos{0} = \frac{1}{2}(e^{0} + e^{-0}) + 1 = \frac{1}{2}(1 + 1) + 1 =
            \frac{1}{2}2 + 1 = 1 + 1 = 2\]

\[v'''(x) = 6\]
\[v'''(0) = 6\]

\[\lim_{x\to 0}{\frac{\sinh{x} - \sin{x}}{x^{3}}} = \lim_{x\to 0}{\frac{u'(x)}{v'(x)}}\]
\[\lim_{x\to 0}{\frac{u'(x)}{v'(x)}} = \lim_{x\to 0}{\frac{u''(x)}{v''(x)}} =
\lim_{x\to 0}{\frac{u'''(x)}{v'''(x)}} = \frac{2}{6} = \frac{1}{3}\]

Result:
\[\lim_{x\to 0}{\frac{\sinh{x} - \sin{x}}{x^{3}}} = \frac{1}{3}\]

\end{document}
