\documentclass[a4paper, 10pt]{scrartcl}

\usepackage[latin1]{inputenc}

\begin{document}

\section{Exercise 892a}

Given:
\[
y = a\sqrt{\cos{2\phi}}
\]

Solution:
\[
y' = a\frac{(-\sin{2\phi})2}{2\sqrt{\cos{2\phi}}} = -a\frac{\sin{2\phi}}{\sqrt{\cos{2\phi}}}
\]

Result:
\[
y' = -a\frac{\sin{2\phi}}{\sqrt{\cos{2\phi}}}
\]

\section{Exercise 892b}

Given:
\[
y = \sqrt{2\phi + \cos^{2}{(2\phi + \frac{\pi}{4})}}
\]

Solution:
\[
y' = \frac{2 + 2\cdot2\cos{(2\phi + \frac{\pi}{4})}(-\sin{(2\phi + \frac{\pi}{4})})}{2\sqrt{2\phi + \cos^{2}{(2\phi + \frac{\pi}{4})}}} =
\]
\[
\frac{1 - 2\cos{(2\phi + \frac{\pi}{4})}\sin{(2\phi + \frac{\pi}{4})}}{\sqrt{2\phi + \cos^{2}{(2\phi + \frac{\pi}{4})}}}
\]

Using: $\sin{2\alpha} = 2\sin{\alpha}\cos{\alpha}$

\[
y' = \frac{1 - 2\cos{(2\phi + \frac{\pi}{4})}\sin{(2\phi + \frac{\pi}{4})}}{\sqrt{2\phi + \cos^{2}{(2\phi + \frac{\pi}{4})}}} =
\]
\[
\frac{1 - \sin{(2(2\phi + \frac{\pi}{4}))}}{\sqrt{2\phi + \cos^{2}{(2\phi + \frac{\pi}{4})}}} =
\]
\[
\frac{1 - \sin{(4\phi + \frac{\pi}{2})}}{\sqrt{2\phi + \cos^{2}{(2\phi + \frac{\pi}{4})}}}
\]

Using:
\[
\sin{(4\phi + \frac{\pi}{2})} = \sin{4\phi}\cos{\frac{\pi}{2}} + \cos{4\phi}\sin{\frac{\pi}{2}} =
\]
\[
\sin{4\phi}\cdot0 + \cos{4\phi}\cdot1 = \cos{4\phi}
\]

\[
y' = \frac{1 - \cos{4\phi}}{\sqrt{2\phi + \cos^{2}{(2\phi + \frac{\pi}{4})}}} =
\frac{1 - \cos{(2\cdot2\phi)}}{\sqrt{2\phi + \cos^{2}{(2\phi + \frac{\pi}{4})}}} =
\]
\[
\frac{2\cdot\frac{1}{2}(1 - \cos{(2\cdot2\phi)})}{\sqrt{2\phi + \cos^{2}{(2\phi + \frac{\pi}{4})}}}
\]

Using: $\sin^{2}{\alpha} = \frac{1}{2}(1 - \cos{2\alpha})$

\[
y' = \frac{2\sin^{2}{2\phi}}{\sqrt{2\phi + \cos^{2}{(2\phi + \frac{\pi}{4})}}}
\]

Result:
\[
y' = \frac{2\sin^{2}{2\phi}}{\sqrt{2\phi + \cos^{2}{(2\phi + \frac{\pi}{4})}}}
\]

\end{document}
