\documentclass[a4paper, 10pt]{scrartcl}

\usepackage[latin1]{inputenc}

\newcommand*\deriv{\mathrm{d}}

\begin{document}

\section{Exercise 1019}

Given:
\[
s = \frac{1}{t\ln{ct}}
\]
\[
t\frac{\deriv s}{\deriv t} + s = -ts^{2}
\]

Solution:
\[
s = \frac{1}{t\ln{ct}} = (t\ln{ct})^{-1}
\]

\[
\frac{\deriv s}{\deriv t} = -1(t\ln{ct})^{-1 - 1}(1\ln{ct} + t\frac{1}{t}) = -\frac{\ln{ct} + 1}{(t\ln{ct})^{2}}
\]

\[
t\left(-\frac{\ln{ct} + 1}{(t\ln{ct})^{2}}\right) + \frac{1}{t\ln{ct}} = -t\left(\frac{1}{t\ln{ct}}\right)^{2}
\]
\[
\frac{-t\ln{ct} - t}{(t\ln{ct})^{2}} + \frac{1}{t\ln{ct}} = \frac{-t}{(t\ln{ct})^{2}}
\]
\[
\frac{-t\ln{ct} - t}{(t\ln{ct})^{2}} + \frac{1}{t\ln{ct}} + \frac{t}{(t\ln{ct})^{2}} = 0
\]
\[
\frac{-t\ln{ct} - t}{(t\ln{ct})^{2}} + \frac{t}{(t\ln{ct})^{2}} + \frac{1}{t\ln{ct}}= 0
\]
\[
\frac{-t\ln{ct} - t + t}{(t\ln{ct})^{2}} + \frac{1}{t\ln{ct}}= 0
\]
\[
\frac{-t\ln{ct}}{(t\ln{ct})^{2}} + \frac{1}{t\ln{ct}}= 0
\]
\[
\frac{-t\ln{ct} + t\ln{ct}}{(t\ln{ct})^{2}} = 0
\]
\[
\frac{0}{(t\ln{ct})^{2}} = 0
\]
\[
0 = 0
\]

\end{document}
