\documentclass[a4paper, 10pt]{scrartcl}

\usepackage[latin1]{inputenc}

\begin{document}

\section{Exercise 36.5}

Given:
\[\lim_{\theta \to 0}{\frac{\sin{\theta} - \theta\cos{\theta}}{\theta^{3}}}\]

Solution:
\[u(\theta) = \sin{\theta} - \theta\cos{\theta}\]
\[u(0) = \sin{0} - 0\cos{0} = 0 - 0 = 0\]

\[v(\theta) = \theta^{3}\]
\[v(0) = 0^{3} = 0\]

\[u'(\theta) = \cos{\theta} - (\theta(-\sin{\theta}) + \cos{\theta}) =
               \cos{\theta} - (-\theta\sin{\theta} + \cos{\theta})\]

\[u'(\theta) = \cos{\theta} + \theta\sin{\theta} - \cos{\theta} = \theta\sin{\theta}\]
\[u'(0) = 0\sin{0} = 0\]

\[v'(\theta) = 3\theta^{3 - 1} = 3\theta^{2}\]
\[v'(0) = 3\cdot 0^{2} = 0\]

\[u''(\theta) = \theta\cos{\theta} + \sin{\theta}\]
\[u''(0) = 0\cos{0} + \sin{0} = 0\]

\[v''(\theta) = 3\cdot 2\theta^{2 - 1} = 6\theta\]
\[v''(0) = 6\cdot 0 = 0\]

\[u'''(\theta) = \theta(-\sin{\theta}) + \cos{\theta} + \cos{\theta} =
                 -\theta\sin{\theta} + 2\cos{\theta} = 2\cos{\theta} - \theta\sin{\theta}\]
\[u'''(0) = 2\cos{0} - 0\sin{0} = 2\cdot 1 - 0 = 2\]

\[v'''(\theta) = 6\]
\[v'''(0) = 6\]

\[\lim_{\theta \to 0}{\frac{u'''(\theta)}{v'''(\theta)}} = \frac{2}{6} = \frac{1}{3}\]

Result:
\[\lim_{\theta \to 0}{\frac{\sin{\theta} - \theta\cos{\theta}}{\theta^{3}}} = \frac{1}{3}\]

\end{document}
