\documentclass[a4paper, 10pt]{scrartcl}

\usepackage[latin1]{inputenc}

\begin{document}

\section{Exercise 64.2}

Given:
\[4\sin{\omega t} - 3\cos{\omega t} = R\sin{(\omega t + \alpha)}\]

Using:
\[\sin{(\alpha + \beta)} = \sin{\alpha}\cos{\beta} + \cos{\alpha}\sin{\beta}\]

Computation of $R$:
\[R\sin{(\omega t + \alpha)} =
R(\sin{\omega t}\cos{\alpha} + \cos{\omega t}\sin{\alpha})\]
\[R\sin{\omega t}\cos{\alpha} + R\cos{\omega t}\sin{\alpha}\]
\[R\cos{\alpha}\sin{\omega t} + R\sin{\alpha}\cos{\omega t}\]

\[R\cos{\alpha} = 4\]
\[\cos{\alpha} = \frac{4}{R}\]

\[R\sin{\alpha} = -3\]
\[\sin{\alpha} = \frac{-3}{R}\]

\[\sin^{2}{\alpha} + \cos^{2}{\alpha} = 1\]
\[\left(\frac{-3}{R}\right)^{2} + \left(\frac{4}{R}\right)^{2} = 1\]
\[\frac{(-3)^{2}}{R^{2}} + \frac{4^{2}}{R^{2}} = 1\]
\[(-3)^{2} + 4^{2} = R^{2}\]
\[R = \sqrt{(-3)^{2} + 4^{2}} = 5\]

Computation of $\alpha$:
\[\tan{\alpha} = \frac{\sin{\alpha}}{\cos{\alpha}}\]
\[\tan{\alpha} = \frac{\frac{-3}{R}}{\frac{4}{R}}\]
\[\tan{\alpha} = \frac{-3}{4}\]
\[\alpha = \arctan{\frac{-3}{4}} \approx -36,8699^\circ \approx -0,6435\textnormal{ rad}\]

Result:
\[4\sin{\omega t} - 3\cos{\omega t} = R\sin{(\omega t + \alpha)} \approx
5\sin{(\omega t - 0,6435)}\]

\end{document}
