\documentclass[a4paper, 10pt]{scrartcl}

\usepackage[latin1]{inputenc}

\begin{document}

\section{Exercise 67.2}

\[f(\theta) = \frac{1}{2}(\sin{9\theta} - \sin{7\theta})\]

Using:
\[\sin{\alpha} - \sin{\beta} = 2\cos{\frac{\alpha + \beta}{2}}\sin{\frac{\alpha - \beta}{2}}\]

\[f(\theta) = \frac{1}{2}(2\cos{\frac{9\theta + 7\theta}{2}}\sin{\frac{9\theta - 7\theta}{2}})\]
\[f(\theta) = \cos{\frac{9\theta + 7\theta}{2}}\sin{\frac{9\theta - 7\theta}{2}}\]
\[f(\theta) = \cos{\frac{16\theta}{2}}\sin{\frac{2\theta}{2}}\]
\[f(\theta) = \cos{8\theta}\sin{\theta}\]

Solution:
\[f(\theta) = \frac{1}{2}(\sin{9\theta} - \sin{7\theta}) = \cos{8\theta}\sin{\theta}\]

\section{Exercise 67.3}

\[f(t) = \cos{5t} + \cos{3t}\]

Using:
\[\cos{\alpha} + \cos{\beta} = 2\cos{\frac{\alpha + \beta}{2}}\cos{\frac{\alpha - \beta}{2}}\]

\[f(t) = 2\cos{\frac{5t + 3t}{2}}\cos{\frac{5t - 3t}{2}}\]
\[f(t) = 2\cos{\frac{8t}{2}}\cos{\frac{2t}{2}}\]
\[f(t) = 2\cos{4t}\cos{t}\]

Solution:
\[f(t) = \cos{5t} + \cos{3t} = 2\cos{4t}\cos{t}\]

\end{document}
