\documentclass[a4paper, 10pt]{scrartcl}

\usepackage[latin1]{inputenc}

\begin{document}

\section{Exercise 1050b}

Given:
\[
ax + by - xy = c
\]

Solution:
\[
a + by' - (y + xy') = 0
\]
\[
a + by' - y - xy' = 0
\]
\[
by' - xy' = y - a
\]
\[
y'(b - x) = y - a
\]
\[
y' = \frac{y - a}{b - x}
\]

\[
y'' = \frac{y'(b - x) - (y - a)(-1)}{(b - x)^{2}} = \frac{y'(b - x) + y - a}{(b - x)^{2}}
\]
\[
y'' = \frac{\frac{y - a}{b - x}(b - x) + y - a}{(b - x)^{2}} = \frac{y - a + y - a}{(b - x)^{2}} = \frac{2(y - a)}{(b - x)^{2}}
\]

Result:
\[
y'' = \frac{2(y - a)}{(b - x)^{2}}
\]

\end{document}
