\documentclass[a4paper, 10pt]{scrartcl}

\usepackage[latin1]{inputenc}

\begin{document}

\section{Exercise 853a}

Given:
\[
y = x + \frac{1}{x^{2}} - \frac{1}{5x^{5}}
\]

Solution:
\[
y = x + \frac{1}{x^{2}} - \frac{1}{5x^{5}} = x + x^{-2} - \frac{1}{5}x^{-5}
\]

\[
y' = 1 + (-2)x^{-2 - 1} - \frac{1}{5}\cdot(-5)x^{-5 - 1} = 1 - 2x^{-3} + x^{-6} = (1 - x^{-3})^{2}
\]

Result:
\[
y' = (1 - x^{-3})^{2}
\]

\section{Exercise 853b}

Given:
\[
y = 3x - 6\sqrt{x}
\]

Solution:
\[
y' = 3 - 6\frac{1}{2\sqrt{x}} = 3 - 3\frac{1}{\sqrt{x}} = 3(1 - \frac{1}{\sqrt{x}})
\]

Result:
\[
y' = 3(1 - \frac{1}{\sqrt{x}})
\]

\end{document}
