\documentclass[a4paper, 10pt]{scrartcl}

\usepackage[latin1]{inputenc}

\begin{document}

\section{Exercise 69.5}

Given:
\[f(t) = e^{t}\ln{t}\cos{t}\]

Solution:
\[u(t) = e^{t}\ln{t}\]
\[u_{0}(t) = e^{t}\]
\[u_{0}'(t) = e^{t}\]
\[v_{0}(t) = \ln{t}\]
\[v_{0}'(t) = \frac{1}{t}\]
\[u'(t) = u_{0}(t)v_{0}'(t) + u_{0}'(t)v_{0}(t) =
          e^{t}\frac{1}{t} + e^{t}\ln{t} =
          e^{t}(\frac{1}{t} + \ln{t})\]

\[v(t) = \cos{t}\]
\[v'(t) = -\sin{t}\]

\[f'(t) = u(t)v'(t) + u'(t)v(t) = e^{t}\ln{t}(-\sin{t}) + e^{t}(\frac{1}{t} + \ln{t})\cos{t}\]
\[f'(t) = e^{t}(\frac{1}{t} + \ln{t})\cos{t} - e^{t}\ln{t}\sin{t}\]
\[f'(t) = e^{t}\left((\frac{1}{t} + \ln{t})\cos{t} - \ln{t}\sin{t}\right)\]
\[f'(t) = e^{t}\left(\frac{\cos{t}}{t} + \ln{t}\cos{t} - \ln{t}\sin{t}\right)\]
\[f'(t) = e^{t}\left(\frac{\cos{t}}{t} + \ln{t}(\cos{t} - \sin{t})\right)\]

Result:
\[f'(t) = e^{t}\left(\frac{\cos{t}}{t} + \ln{t}(\cos{t} - \sin{t})\right)\]

\end{document}
