\documentclass[a4paper, 10pt]{scrartcl}

\usepackage[latin1]{inputenc}

\begin{document}

\section{Exercise 36.4}

Given:
\[\lim_{x\to 0}{\frac{x^{2} - \sin{3x}}{3x + x^{2}}}\]

Solution:
\[u(x) = x^{2} - \sin{3x}\]
\[u(0) = 0^{2} - \sin{3\cdot 0} = -\sin{0} = 0\]

\[v(x) = 3x + x^{2}\]
\[v(0) = 3\cdot 0 + 0^{2} = 0\]

\[u'(x) = 2x^{2 - 1} - 3\cos{3x} = 2x^{1} - 3\cos{3x} = 2x - 3\cos{3x}\]
\[u'(0) = 2\cdot 0 - 3\cos{3\cdot 0} = -3\cos{0} = -3 \cdot 1 = -3\]

\[v'(x) = 3 + 2x^{2 - 1} = 3 + 2x^{1} = 3 + 2x\]
\[v'(0) = 3 + 2\cdot 0 = 3\]

\[\lim_{x\to 0}{\frac{x^{2} - \sin{3x}}{3x + x^{2}}} = \lim_{x\to 0}{\frac{u'(x)}{v'(x)}}\]
\[\lim_{x\to 0}{\frac{u'(x)}{v'(x)}} = \frac{-3}{3} = -1\]

Result:
\[\lim_{x\to 0}{\frac{x^{2} - \sin{3x}}{3x + x^{2}}} = -1\]

\end{document}
