\documentclass[a4paper, 10pt]{scrartcl}

\usepackage[latin1]{inputenc}

\begin{document}

\section{Exercise 769}

Given:
\[\lim_{h\to 0}{\frac{\sin{(x + h)} - \sin{(x - h)}}{h}}\]

Solution:
\[u(h) = \sin{(x + h)} - \sin{(x - h)}\]
\[u(0) = \sin{(x + 0)} - \sin{(x - 0)} = \sin{x} - \sin{x} = 0\]

\[v(h) = h\]
\[v(0) = 0\]

\[u'(h) = \cos{(x + h)} - (-\cos{(x - h)}) = \cos{(x + h)} + \cos{(x - h)}\]
\[u'(0) = \cos{(x + 0)} + \cos{(x - 0)} = \cos{x} + \cos{x} = 2\cos{x}\]

\[v'(h) = 1\]
\[v'(0) = 1\]

\[\lim_{h\to 0}{\frac{\sin{(x + h)} - \sin{(x - h)}}{h}} = \lim_{h\to 0}{\frac{u'(h)}{v'(h)}} =
\frac{2\cos{x}}{1} = 2\cos{x}\]

Result:
\[\lim_{h\to 0}{\frac{\sin{(x + h)} - \sin{(x - h)}}{h}} = 2\cos{x}\]

\end{document}
