\documentclass[a4paper, 10pt]{scrartcl}

\usepackage[latin1]{inputenc}

\begin{document}

\section{Exercise 65.2a}

Given:
\[1 - \frac{\cos{2\phi}}{\cos^{2}{\phi}} = \tan^{2}{\phi}\]

Using:
\[\cos{2\alpha} = 2\cos^{2}{\alpha} - 1\]

Solution:
\[1 - \frac{\cos{2\phi}}{\cos^{2}{\phi}} = 1 - \frac{2\cos^{2}{\phi} - 1}{\cos^{2}{\phi}} =
1 - \left(\frac{2\cos^{2}{\phi}}{\cos^{2}{\phi}} - \frac{1}{\cos^{2}{\phi}}\right) =
1 - (2 - \frac{1}{\cos^{2}{\phi}})\]

\[1 - 2 + \frac{1}{\cos^{2}{\phi}} =
\frac{1}{\cos^{2}{\phi}} - 1 =
\frac{1 - \cos^{2}{\phi}}{\cos^{2}{\phi}}\]

Using:
\[\cos^{2}{\alpha} + \sin^{2}{\alpha} = 1\]
\[\sin^{2}{\alpha} = 1 - \cos^{2}{\alpha}\]

\[\frac{1 - \cos^{2}{\phi}}{\cos^{2}{\phi}} = \frac{\sin^{2}{\phi}}{\cos^{2}{\phi}} =
\tan^{2}{\phi}\]

\section{Exercise 65.2b}

Given:
\[\frac{1 + \cos{2t}}{\sin^{2}{t}} = 2\cot^{2}{t}\]

Using:
\[\cos{2\alpha} = 2\cos^{2}{\alpha} - 1\]

\[\frac{1 + 2\cos^{2}{t} - 1}{\sin^{2}{t}} = \frac{2\cos^{2}{t}}{\sin^{2}{t}} = 2\cot^{2}{t}\]

\end{document}
