\documentclass[a4paper, 10pt]{scrartcl}

\usepackage[latin1]{inputenc}

\begin{document}

\section{Exercise 1046a}

Given:
\[
x^{\frac{2}{3}} + y^{\frac{2}{3}} = a^{\frac{2}{3}}
\]

Solution:
\[
\frac{2}{3}x^{\frac{2}{3} - 1} + \frac{2}{3}y^{\frac{2}{3} - 1}y' = 0
\]
\[
\frac{2}{3}x^{-\frac{1}{3}} + \frac{2}{3}y^{-\frac{1}{3}}y' = 0
\]
\[
x^{-\frac{1}{3}} + y^{-\frac{1}{3}}y' = 0
\]
\[
y^{-\frac{1}{3}}y' = -x^{-\frac{1}{3}}
\]
\[
y' = -\frac{x^{-\frac{1}{3}}}{y^{-\frac{1}{3}}} = -\frac{y^{\frac{1}{3}}}{x^{\frac{1}{3}}} = -\frac{\sqrt[3]{y}}{\sqrt[3]{x}}
= -\sqrt[3]{\frac{y}{x}}
\]

Result:
\[
y'= -\sqrt[3]{\frac{y}{x}}
\]

\end{document}
